language_formal/spark2014_semantics/semantics.v
@@ -65,7 +65,9 @@ Inductive eval_bin_expr: binary_operator -> value -> value -> value -> Prop :=
 Inductive eval_unary_expr : unary_operator -> value -> value -> Prop :=
     | Unary_Not: forall b v,
         negb b = v ->
-        eval_unary_expr Not (Bool b) (Bool v).
+        eval_unary_expr Not (Bool b) (Bool v)
+    | EUnary_Plus: forall v,
+        eval_unary_expr Unary_Plus (Int v) (Int v).
 
 Lemma eval_bin_unique: forall op v1 v2 x y,
     eval_bin_expr op v1 v2 x ->
@@ -102,38 +104,38 @@ Qed.
     normal binary operation result is returned;
 *)
 
-Inductive eval_expr: store -> expression -> return_val -> Prop :=
+Inductive eval_expr: stack -> expression -> Return value -> Prop :=
     | eval_E_Literal: forall l v s ast_num,
         eval_literal l = v ->
-        eval_expr s (E_Literal ast_num l) (Val_Normal v)
+        eval_expr s (E_Literal ast_num l) (Normal v)
     | eval_E_Identifier: forall x s v ast_num,
-        fetch x s = Some (Value v) ->
-        eval_expr s (E_Identifier ast_num x) (Val_Normal v)
+        fetchG x s = Some (Value v) ->
+        eval_expr s (E_Identifier ast_num x) (Normal v)
     | eval_E_Binary_Operation1: forall s e1 ast_num op e2,
-        eval_expr s e1 Val_Run_Time_Error ->
-        eval_expr s (E_Binary_Operation ast_num op e1 e2) Val_Run_Time_Error
+        eval_expr s e1 Run_Time_Error ->
+        eval_expr s (E_Binary_Operation ast_num op e1 e2) Run_Time_Error
     | eval_E_Binary_Operation2: forall s e1 v1 e2 ast_num op,
-        eval_expr s e1 (Val_Normal v1) ->
-        eval_expr s e2 Val_Run_Time_Error ->
-        eval_expr s (E_Binary_Operation ast_num op e1 e2) Val_Run_Time_Error
+        eval_expr s e1 (Normal v1) ->
+        eval_expr s e2 Run_Time_Error ->
+        eval_expr s (E_Binary_Operation ast_num op e1 e2) Run_Time_Error
     | eval_E_Binary_Operation3: forall s e1 v1 e2 v2 ast_num op,
-        eval_expr s e1 (Val_Normal v1) ->
-        eval_expr s e2 (Val_Normal v2) ->
+        eval_expr s e1 (Normal v1) ->
+        eval_expr s e2 (Normal v2) ->
         do_check op v1 v2 false ->
-        eval_expr s (E_Binary_Operation ast_num op e1 e2) Val_Run_Time_Error
+        eval_expr s (E_Binary_Operation ast_num op e1 e2) Run_Time_Error
     | eval_E_Binary_Operation4: forall s e1 v1 e2 v2 ast_num op v,
-        eval_expr s e1 (Val_Normal v1) ->
-        eval_expr s e2 (Val_Normal v2) ->
+        eval_expr s e1 (Normal v1) ->
+        eval_expr s e2 (Normal v2) ->
         do_check op v1 v2 true ->
         eval_bin_expr op v1 v2 v ->
-        eval_expr s (E_Binary_Operation ast_num op e1 e2) (Val_Normal v)
+        eval_expr s (E_Binary_Operation ast_num op e1 e2) (Normal v)
     | eval_E_Unary_Operation1: forall s e ast_num op,
-        eval_expr s e Val_Run_Time_Error ->
-        eval_expr s (E_Unary_Operation ast_num op e) Val_Run_Time_Error
+        eval_expr s e Run_Time_Error ->
+        eval_expr s (E_Unary_Operation ast_num op e) Run_Time_Error
     | eval_E_Unary_Operation2: forall s e v ast_num op v1,
-        eval_expr s e (Val_Normal v) ->
+        eval_expr s e (Normal v) ->
         eval_unary_expr op v v1 ->
-        eval_expr s (E_Unary_Operation ast_num op e) (Val_Normal v1).
+        eval_expr s (E_Unary_Operation ast_num op e) (Normal v1).
 
 
 
@@ -158,14 +160,14 @@ Inductive eval_expr: store -> expression -> return_val -> Prop :=
     the body of the procedure;
   - [s'] is the resulting state. *)
 Inductive Copy_out: store -> list parameter_specification
-                    -> list expression -> store -> store -> Prop :=
+                    -> list expression -> stack -> stack -> Prop :=
   Copy_out_nil : forall prf σ, Copy_out prf nil nil σ σ
 | Copy_out_cons_out:
     forall σ σ' σ'' id v prf prm lprm lexp idorig astnum,
       prm.(parameter_mode) = Out
       -> id = prm.(parameter_name)
       -> fetch id prf = Some v
-      -> update σ idorig v = Some σ'
+      -> updateG σ idorig v = Some σ'
       -> Copy_out prf lprm lexp σ' σ''
       -> Copy_out prf (prm::lprm) ((E_Identifier astnum idorig) :: lexp) σ σ''
 | Copy_out_cons_in:
@@ -180,76 +182,80 @@ Inductive Copy_out: store -> list parameter_specification
     parameters described by [lpamrams]. these values are computed from
     the list of arguments [lexp]. Only "In" parameters are evaluated,
     "Out" parameters are set to [Undefined]. *)
-Inductive Copy_in: store -> list parameter_specification
-                   -> list expression -> state -> Prop :=
-  Copy_in_nil : forall σ, Copy_in σ nil nil (S_Normal nil) 
+Inductive Copy_in: stack -> list parameter_specification
+                   -> list expression -> Return store -> Prop :=
+  Copy_in_nil : forall σ, Copy_in σ nil nil (Normal nil) 
 | Copy_in_cons_out:
-    forall σ lparam lexp frame prm idv ast_num,
-      Copy_in σ lparam lexp (S_Normal frame)
+    forall σ lparam lexp (frame:store) prm idv ast_num,
+      Copy_in σ lparam lexp (Normal frame)
       -> prm.(parameter_mode) = Out
       -> Copy_in σ (prm::lparam) (E_Identifier ast_num idv::lexp)
-                 (S_Normal ((prm.(parameter_name),Undefined)::frame))
+                 (Normal ((prm.(parameter_name),Undefined)::frame))
 | Copy_in_cons_out_rte:
     forall σ lparam lexp prm idv ast_num,
-      Copy_in σ lparam lexp S_Run_Time_Error
+      Copy_in σ lparam lexp Run_Time_Error
       -> prm.(parameter_mode) = Out
-      -> Copy_in σ (prm::lparam) (E_Identifier ast_num idv::lexp) S_Run_Time_Error
+      -> Copy_in σ (prm::lparam) (E_Identifier ast_num idv::lexp) Run_Time_Error
 | Copy_in_cons_in_rte1:
     forall σ lparam lexp prm e,
       prm.(parameter_mode) = In
-      -> eval_expr σ e Val_Run_Time_Error
-      -> Copy_in σ (prm::lparam) (e::lexp) S_Run_Time_Error
+      -> eval_expr σ e Run_Time_Error
+      -> Copy_in σ (prm::lparam) (e::lexp) Run_Time_Error
 | Copy_in_cons_in_rte2:
     forall σ lparam lexp prm e v,
-      Copy_in σ lparam lexp S_Run_Time_Error
-      -> eval_expr σ e (Val_Normal v)
+      Copy_in σ lparam lexp Run_Time_Error
+      -> eval_expr σ e (Normal v)
       -> prm.(parameter_mode) = In
-      -> Copy_in σ (prm::lparam) (e::lexp) S_Run_Time_Error
+      -> Copy_in σ (prm::lparam) (e::lexp) Run_Time_Error
 | Copy_in_cons_in:
     forall σ lparam lexp frame prm e v,
-      Copy_in σ lparam lexp (S_Normal frame)
+      Copy_in σ lparam lexp (Normal frame)
       -> prm.(parameter_mode) = In
-      -> eval_expr σ e (Val_Normal v)
+      -> eval_expr σ e (Normal v)
       -> Copy_in σ (prm::lparam) (e::lexp)
-                 (S_Normal ((prm.(parameter_name),Value v)::frame)).
+                 (Normal ((prm.(parameter_name),Value v)::frame)).
 
 
-(** *** Inductive semantic of declarations *)
-Inductive eval_decl: store -> declaration -> state -> Prop :=
+(** *** Inductive semantic of declarations. [eval_decl s nil decl
+        rsto] means that rsto is the frame to be pushed on s after
+        evaluating decl, sto is used as an accumulator for building
+        the frame.
+ *)
+Inductive eval_decl: stack -> store -> declaration -> Return store -> Prop :=
 | eval_Decl_E:
-    forall e d s,
+    forall e d s sto,
       Some e = d.(initialization_expression) ->
-      eval_expr s e Val_Run_Time_Error ->
-      eval_decl s (D_Object_declaration d) S_Run_Time_Error
+      eval_expr (sto::s) e Run_Time_Error ->
+      eval_decl s sto (D_Object_declaration d) Run_Time_Error
 | eval_Decl:
-    forall d x e v s,
+    forall d x e v s sto,
       x = d.(object_name) ->
       Some e = d.(initialization_expression) ->
-      eval_expr s e (Val_Normal v) ->
-      eval_decl s (D_Object_declaration d) (S_Normal ((x, Value v) :: s))
+      eval_expr (sto::s) e (Normal v) ->
+      eval_decl s sto (D_Object_declaration d) (Normal ((x, Value v) :: sto))
 | eval_UndefDecl:
-    forall d x s,
+    forall d x s sto,
       x = d.(object_name) ->
       None = d.(initialization_expression) ->
-      eval_decl s (D_Object_declaration d) (S_Normal ((x, Undefined) :: s))
+      eval_decl s sto (D_Object_declaration d) (Normal ((x, Undefined) :: sto))
 | eval_decl_Seq:
-    forall dcl1 dcl2 s s' s'',
-      eval_decl s dcl1 (S_Normal s') ->
-      eval_decl s' dcl2 (S_Normal s'') ->
-      eval_decl s (D_Sequence dcl1 dcl2) (S_Normal s'')
+    forall dcl1 dcl2 s s' s'' sto,
+      eval_decl s sto dcl1 (Normal s') ->
+      eval_decl s s' dcl2 (Normal s'') ->
+      eval_decl s sto (D_Sequence dcl1 dcl2) (Normal s'')
 | eval_decl_Seq_err1:
-    forall dcl1 dcl2 s,
-      eval_decl s dcl1 S_Run_Time_Error ->
-      eval_decl s (D_Sequence dcl1 dcl2) S_Run_Time_Error
+    forall dcl1 dcl2 s sto,
+      eval_decl s sto dcl1 Run_Time_Error ->
+      eval_decl s sto (D_Sequence dcl1 dcl2) Run_Time_Error
 | eval_decl_Seq_err2:
-    forall dcl1 dcl2 s s',
-      eval_decl s dcl1 (S_Normal s') ->
-      eval_decl s' dcl2 S_Run_Time_Error ->
-      eval_decl s (D_Sequence dcl1 dcl2) S_Run_Time_Error
+    forall dcl1 dcl2 s s' sto,
+      eval_decl s sto dcl1 (Normal s') ->
+      eval_decl s s' dcl2 Run_Time_Error ->
+      eval_decl s sto (D_Sequence dcl1 dcl2) Run_Time_Error
 | eval_decl_proc:
-    forall s pbody,
-      eval_decl s (D_Procedure_declaration pbody)
-                (S_Normal ((procedure_name pbody,Procedure pbody)::s)).
+    forall s pbody sto,
+      eval_decl s sto (D_Procedure_declaration pbody)
+                (Normal ((procedure_name pbody,Procedure pbody)::sto)).
 
 (** ** Inductive semantic of statement and declaration
 
@@ -260,81 +266,75 @@ Inductive eval_decl: store -> declaration -> state -> Prop :=
 
  *)
 
-Inductive eval_stmt: store -> statement -> state -> Prop := 
+Inductive eval_stmt: stack -> statement -> Return stack -> Prop := 
     | eval_S_Assignment1: forall s e ast_num x,
-        eval_expr s e Val_Run_Time_Error ->
-        eval_stmt s (S_Assignment ast_num x e) S_Run_Time_Error
+        eval_expr s e Run_Time_Error ->
+        eval_stmt s (S_Assignment ast_num x e) Run_Time_Error
     | eval_S_Assignment2: forall s e v x s1 ast_num,
-        eval_expr s e (Val_Normal v) ->
-        update s x (Value v) = Some s1 ->
-        eval_stmt s (S_Assignment ast_num x e) (S_Normal s1)
+        eval_expr s e (Normal v) ->
+        updateG s x (Value v) = Some s1 ->
+        eval_stmt s (S_Assignment ast_num x e) (Normal s1)
     | eval_S_Sequence1: forall s c1 ast_num c2,
-        eval_stmt s c1 S_Run_Time_Error ->
-        eval_stmt s (S_Sequence ast_num c1 c2) S_Run_Time_Error
+        eval_stmt s c1 Run_Time_Error ->
+        eval_stmt s (S_Sequence ast_num c1 c2) Run_Time_Error
     | eval_S_Sequence2: forall ast_num s s1 s2 c1 c2,
-        eval_stmt s c1 (S_Normal s1) ->
+        eval_stmt s c1 (Normal s1) ->
         eval_stmt s1 c2 s2 ->
         eval_stmt s (S_Sequence ast_num c1 c2) s2
     | eval_S_If: forall s b ast_num c,
-        eval_expr s b Val_Run_Time_Error ->
-        eval_stmt s (S_If ast_num b c) S_Run_Time_Error
+        eval_expr s b Run_Time_Error ->
+        eval_stmt s (S_If ast_num b c) Run_Time_Error
     | eval_S_If_True: forall s b c s1 ast_num,
-        eval_expr s b (Val_Normal (Bool true)) ->
+        eval_expr s b (Normal (Bool true)) ->
         eval_stmt s c s1 ->
         eval_stmt s (S_If ast_num b c) s1
     | eval_S_If_False: forall s b ast_num c,
-        eval_expr s b (Val_Normal (Bool false)) ->
-        eval_stmt s (S_If ast_num b c) (S_Normal s)
+        eval_expr s b (Normal (Bool false)) ->
+        eval_stmt s (S_If ast_num b c) (Normal s)
     | eval_S_While_Loop: forall s b ast_num c,
-        eval_expr s b Val_Run_Time_Error ->
-        eval_stmt s (S_While_Loop ast_num b c) S_Run_Time_Error
+        eval_expr s b Run_Time_Error ->
+        eval_stmt s (S_While_Loop ast_num b c) Run_Time_Error
     | eval_S_While_Loop_True1: forall s b c ast_num,
-        eval_expr s b (Val_Normal (Bool true)) ->
-        eval_stmt s c S_Run_Time_Error ->
-        eval_stmt s (S_While_Loop ast_num b c) S_Run_Time_Error
+        eval_expr s b (Normal (Bool true)) ->
+        eval_stmt s c Run_Time_Error ->
+        eval_stmt s (S_While_Loop ast_num b c) Run_Time_Error
     | eval_S_While_Loop_True2: forall s b c s1 ast_num s2,
-        eval_expr s b (Val_Normal (Bool true)) ->
-        eval_stmt s c (S_Normal s1) ->
+        eval_expr s b (Normal (Bool true)) ->
+        eval_stmt s c (Normal s1) ->
         eval_stmt s1 (S_While_Loop ast_num b c) s2 ->
         eval_stmt s (S_While_Loop ast_num b c) s2
     | eval_S_While_Loop_False: forall s b ast_num c,
-        eval_expr s b (Val_Normal (Bool false)) ->
-        eval_stmt s (S_While_Loop ast_num b c) (S_Normal s)
+        eval_expr s b (Normal (Bool false)) ->
+        eval_stmt s (S_While_Loop ast_num b c) (Normal s)
     | eval_S_Proc_rteargs:
         forall pbname (pb:procedure_body) lexp s ast_num,
-          fetch pbname s = Some (Procedure pb) ->
-          Copy_in s (procedure_parameter_profile pb) lexp S_Run_Time_Error ->
-          eval_stmt s (S_ProcCall ast_num pbname lexp) S_Run_Time_Error
+          fetchG pbname s = Some (Procedure pb) ->
+          Copy_in s (procedure_parameter_profile pb) lexp Run_Time_Error ->
+          eval_stmt s (S_ProcCall ast_num pbname lexp) Run_Time_Error
     | eval_S_Proc_rtedecl:
-        forall pbname (pb:procedure_body) lexp s ast_num s1
-               prefix,
-          fetch pbname s = Some (Procedure pb) ->
-          Copy_in s (procedure_parameter_profile pb) lexp (S_Normal prefix) ->
-          s1 = prefix ++ s ->
-          eval_decl s1 (procedure_declarative_part pb) S_Run_Time_Error ->
-          eval_stmt s (S_ProcCall ast_num pbname lexp) S_Run_Time_Error
+        forall pbname (pb:procedure_body) lexp s ast_num prefix,
+          fetchG pbname s = Some (Procedure pb) ->
+          Copy_in s (procedure_parameter_profile pb) lexp (Normal prefix) ->
+          eval_decl s prefix (procedure_declarative_part pb) Run_Time_Error ->
+          eval_stmt s (S_ProcCall ast_num pbname lexp) Run_Time_Error
     | eval_S_Proc_rtebody:
-        forall pbname (pb:procedure_body) lexp s ast_num s1 s2 
-               prefix,
-          fetch pbname s = Some (Procedure pb) ->
-          Copy_in s (procedure_parameter_profile pb) lexp (S_Normal prefix) ->
-          s1 = prefix ++ s ->
-          eval_decl s1 (procedure_declarative_part pb) (S_Normal s2) ->
-          eval_stmt s2 (procedure_statements pb) S_Run_Time_Error ->
-          eval_stmt s (S_ProcCall ast_num pbname lexp) S_Run_Time_Error
+        forall pbname (pb:procedure_body) lexp s ast_num s2 prefix,
+          fetchG pbname s = Some (Procedure pb) ->
+          Copy_in s (procedure_parameter_profile pb) lexp (Normal prefix) ->
+          eval_decl s prefix (procedure_declarative_part pb) (Normal s2) ->
+          eval_stmt (s2::s) (procedure_statements pb) Run_Time_Error ->
+          eval_stmt s (S_ProcCall ast_num pbname lexp) Run_Time_Error
     | eval_S_Proc:
-        forall pbname (pb:procedure_body) lexp s ast_num s1 s2 s3 s' s'' slocal
+        forall pbname (pb:procedure_body) lexp s ast_num s2 s3 s' s'' slocal
                prefix prefix',
-          fetch pbname s = Some (Procedure pb) ->
-          Copy_in s (procedure_parameter_profile pb) lexp (S_Normal prefix) ->
-          s1 = prefix ++ s ->
-          eval_decl s1 (procedure_declarative_part pb) (S_Normal s2) ->
-          eval_stmt s2 (procedure_statements pb) (S_Normal s3) ->
-          s3 = slocal ++ prefix' ++ s' ->
-          List.length s' = List.length s ->
+          fetchG pbname s = Some (Procedure pb) ->
+          Copy_in s (procedure_parameter_profile pb) lexp (Normal prefix) ->
+          eval_decl s prefix (procedure_declarative_part pb) (Normal s2) ->
+          eval_stmt (s2::s) (procedure_statements pb) (Normal s3) ->
+          s3 = (slocal ++ prefix') :: s' -> (* extract parameters from local frame *)
           List.length prefix = List.length prefix' ->
           Copy_out prefix' (procedure_parameter_profile pb) lexp s' s'' ->
-          eval_stmt s (S_ProcCall ast_num pbname lexp) (S_Normal s'')
+          eval_stmt s (S_ProcCall ast_num pbname lexp) (Normal s'')
 .
 
 
@@ -362,39 +362,1653 @@ Definition proc1:procedure_body := (mkprocedure_body
              )
              (S_Assignment 12 102 (E_Literal 8 (Integer_Literal(56))))).
 
-Definition s1:store := (101,Procedure proc1) :: (102, Value (Int(77))) :: nil.
+Definition s1:stack := ((101,Procedure proc1) :: (102, Value (Int(77))) :: nil)::nil.
 
-Definition s2:store := (101,Procedure proc1) :: (102, Value (Int(56)))  :: nil.
+Definition s2:stack := ((101,Procedure proc1) :: (102, Value (Int(56)))  :: nil)::nil.
 
 
-Lemma essai: eval_stmt s1 (S_ProcCall 13 101 nil) (S_Normal s2).
+Lemma essai: eval_stmt s1 (S_ProcCall 13 101 nil) (Normal s2).
 Proof.
   eapply eval_S_Proc; try now (simpl; eauto).
   - simpl.
     instantiate (1 := nil).
     constructor.
-  - simpl List.app.
-    instantiate (1:= ((4, Value (Int 34))::s1)).
-    unfold s1, s2, proc1.
-    simpl.
-    econstructor 2.
-    + econstructor;eauto.
+  - econstructor 2.
     + reflexivity.
+    + simpl.
+      reflexivity.
     + constructor.
       simpl.
       reflexivity.
-  - instantiate (2:=(4, Value (Int 34))::nil).
-    instantiate (1:=s2).
-    simpl.
+  - simpl.
     econstructor.
     + econstructor.
       simpl.
       eauto.
     + simpl.
+      rewrite app_nil_r.
       reflexivity.
-  - reflexivity.
   - simpl.
     constructor 1.
+Qed.
+
+
+
+(* v102 is a variable in the scope.
+procedure P2 () is
+  V4 : TYPE5 := 34;
+  V5 : TYPE5 := 37;
+begin
+  V5 := V4 + V5;
+  V102 := V5*2;
+end 
+*)
+Definition proc2:procedure_body := (mkprocedure_body
+           1 2 nil nil
+             (D_Sequence
+                (D_Object_declaration
+                   {|
+                     declaration_astnum := 3;
+                     object_name := 4;
+                     object_nominal_subtype :=  5;
+                     initialization_expression := Some (E_Literal 6 (Integer_Literal(34)))
+                   |}
+                )
+                (D_Object_declaration
+                   {|
+                     declaration_astnum := 4;
+                     object_name := 5;
+                     object_nominal_subtype :=  5;
+                     initialization_expression := Some (E_Literal 6 (Integer_Literal(37)))
+                   |}
+                )
+             )
+             (S_Sequence 13
+                (S_Assignment 14 5
+                              (E_Binary_Operation 9 Plus
+                                                  (E_Identifier 10 5)
+                                                  (E_Identifier 10 4)))
+                (S_Assignment
+                   12
+                   102
+                   (E_Binary_Operation 9 Multiply
+                                       (E_Identifier 10 5)
+                                       (E_Literal 8 (Integer_Literal(2))))))).
+
+Definition sto3:store := (101,Procedure proc2) :: (102, Value (Int(77))) :: nil.
+
+Definition sto4:store := (101,Procedure proc2) :: (102, Value (Int(142)))  :: nil.
+
+
+
+Lemma essai2: eval_stmt (sto3::nil) (S_ProcCall 13 101 nil) (Normal (sto4::nil)).
+Proof.
+  eapply eval_S_Proc; try now (simpl; eauto).
+  - simpl.
+    constructor.
+  - 
+(*     instantiate (1:= ((5, Value (Int 37))::(4, Value (Int 34))::s3)). *)
+    unfold sto3, sto4, proc1.
+    simpl.
+    econstructor 4;simpl.
+    + econstructor 2;simpl.
+      * econstructor;eauto.
+      * reflexivity.
+      * constructor.
+        simpl.
+        reflexivity.
+    + econstructor 2;simpl.
+      * econstructor;eauto.
+      * reflexivity.
+      * constructor.
+        simpl.
+        reflexivity.
+  - simpl.
+    + { econstructor.
+        - econstructor.
+          + econstructor.
+            * econstructor.
+              simpl.
+              eauto.
+            * constructor.
+              simpl.
+              eauto.
+            * constructor.
+              vm_compute.
+              reflexivity.
+            * econstructor.
+              simpl.
+              eauto.
+          + simpl.
+            reflexivity.
+        - econstructor.
+          + econstructor.
+            * econstructor.
+              simpl.
+              eauto.
+            * econstructor.
+              simpl.
+              eauto.
+            * econstructor.
+              vm_compute.
+              reflexivity.
+            * econstructor.
+            simpl.
+            eauto.
+        + simpl.
+          rewrite app_nil_r.
+          reflexivity. }
+  - simpl.
+    constructor 1.
+Qed.
+
+
+End ExampleProcedures.
+(* END EXAMPLE *)  
+
+(** ** Functional Semantics of expressions *)
+
+(** for relational semantics of expression and statement, we also 
+    provide its corresponding version of functional semantics, and 
+    prove that they are semantics equivalent;
+    relational semantics encode the formal semantics rules, while
+    functional semantics is useful to familiarize oneself with the 
+    SPARK 2014 semantics, and validate it experimentally by testing, 
+    and it also helps to fix the program if the program exhibits 
+    undefined behavior;
+    
+    Bisimulation between relational and functional semantics are
+    proved for the following pairs of evaluations: 
+    
+    - f_eval_binexpr <-> eval_binexpr;
+    
+    - f_eval_unaryexpr <-> eval_unaryexpr;
+    
+    - f_eval_expr <-> eval_expr;
+
+    - f_eval_stmt <-> eval_stmt;
+*)
+
+(** *** semantic of operators *)
+
+(** interpret the binary operation for each binary operator *)
+Definition f_eval_bin_expr (op: binary_operator) (v1: value) (v2: value): Return value :=
+    match op with
+    | Equal => Val.eq v1 v2
+    | Not_Equal => Val.ne v1 v2
+    | Greater_Than => Val.gt v1 v2
+    | Greater_Than_Or_Equal => Val.ge v1 v2
+    | Less_Than => Val.lt v1 v2
+    | Less_Than_Or_Equal => Val.le v1 v2
+    | And => Val.and v1 v2
+    | Or => Val.or v1 v2
+    | Plus => Val.add v1 v2
+    | Minus => Val.sub v1 v2
+    | Multiply => Val.mul v1 v2
+    | Divide => Val.div v1 v2
+    end.
+
+(** interpret the unary operation *)
+Definition f_eval_unary_expr (op: unary_operator) (v: value): Return value :=
+    match op with
+    | Not => Val.not v
+    | Unary_Plus => Val.unary_add v
+    end.
+
+(** *** Expression semantics *)
+
+(** in functional semantics for expression, it returns either a
+    normal value or a run time error or go abnormal, the run time 
+    checks (for example, division by zero check) are encoded inside 
+    the semantics; *)
+Function f_eval_expr (s: stack) (e: expression): Return value :=
+    match e with
+    | E_Literal _ v => Normal (eval_literal v)
+    | E_Identifier _ x =>
+        match (fetchG x s) with
+        | Some (Value v) => Normal v
+        | _ => Abnormal (* None or procedure *)
+        end
+    | E_Binary_Operation _ op e1 e2 =>
+        match f_eval_expr s e1 with
+        | Normal v1 => 
+            match f_eval_expr s e2 with
+            | Normal v2 => 
+                match f_do_check op v1 v2 with
+                | Some true => f_eval_bin_expr op v1 v2
+                | Some false => Run_Time_Error
+                | _ => Abnormal
+                end
+            | Run_Time_Error => Run_Time_Error
+            | Abnormal => Abnormal
+            | Unterminated => Unterminated
+            end
+        | Run_Time_Error => Run_Time_Error
+        | Abnormal => Abnormal
+        | Unterminated => Unterminated
+        end   
+    | E_Unary_Operation _ op e => 
+        match f_eval_expr s e with
+        | Normal v => f_eval_unary_expr op v
+        | Run_Time_Error => Run_Time_Error
+        | Abnormal => Abnormal
+        | Unterminated => Unterminated
+        end
+    end.
+
+(** ** Functional Statement semantics *)
+
+
+(** *** Functional manipulation of the stack for procedure call and
+    retrun *)
+
+(** functional version of Copy_out
+  [copy_out prefx params lexp s'] returns s' updated in the following
+  way: for each param in params that is Out, pick the correponding
+  variable name in lexp and update s' with the value of the param that
+  is stored in prefix. *)
+Function copy_out (prefx:store) (params: list parameter_specification)
+         (lexp:list expression) (s: stack) {struct params}:  Return stack :=
+  match params, lexp with
+    | nil , nil => Normal s
+    | (prm::params') , (e::lexp') =>
+      match prm.(parameter_mode) with
+         | Out =>
+           match e with
+             | E_Identifier _ x =>
+               match (fetch (prm.(parameter_name)) prefx) with
+                   Some v =>
+                   match updateG s x v with
+                     | Some s' => copy_out prefx params' lexp' s'
+                     | None => Abnormal
+                   end
+                 | None => Abnormal
+               end
+             | _ => Abnormal
+           end
+         | In => copy_out prefx params' lexp' s
+         | _ => Abnormal
+       end
+    | _ , _ => Abnormal
+  end.
+
+(** Functional version of Copy_in.
+   [copy_in s lparams lexp] returns the prefix to push on the stack
+   before evaluationg procedure body (i.e. declaration block +
+   statement). "Out" parameters values are copied into there output
+   variables (stored in lexp). *)
+Function copy_in (s:stack) lparams lexp: Return store :=
+  match lparams,lexp with
+  | (prm :: lparams') , (exp:: lexp') =>
+    match prm.(parameter_mode) with
+      | Out => if is_var exp
+               then match copy_in s lparams' lexp' with
+                      | Normal res => Normal ((prm.(parameter_name), Undefined) :: res)
+                      | res => res
+                    end
+               else Abnormal
+      | In =>
+        let v := f_eval_expr s exp in
+        match v with
+          | Normal v' =>
+            match copy_in s lparams' lexp' with
+              | Normal res => Normal ((prm.(parameter_name), Value v') :: res)
+              | res => res
+            end
+          | Run_Time_Error => Run_Time_Error
+          | Abnormal => Abnormal
+          | Unterminated => Unterminated
+        end
+      | In_Out => Abnormal (* not yet implemented *)
+    end
+  | nil , nil => Normal nil
+  | _ , _ => Abnormal
+  end.
+
+(** *** functional semantic of declarations *)
+
+Function f_eval_decl (s: stack) (sto:store) (c: declaration) {struct c}: Return store :=
+  match c with
+    | D_Object_declaration d =>
+      match d.(initialization_expression) with
+        | Some e =>
+          match f_eval_expr (sto::s) e with
+            | Run_Time_Error => Run_Time_Error
+            | Normal v =>
+              (Normal ((d.(object_name), Value v)::sto))
+            | Abnormal => Abnormal
+            | Unterminated => Unterminated
+          end
+        | None => (Normal ((d.(object_name), Undefined) :: sto))
+      end
+    | D_Sequence dcl1 dcl2 =>
+      match f_eval_decl s sto dcl1 with
+        | Normal s' => f_eval_decl s s' dcl2
+        | err => err
+      end
+    | D_Procedure_declaration pbody =>
+      Normal((procedure_name pbody,Procedure pbody)::sto)
+  end.
+
+(** *** functional semantic of statements *)
+
+(** 
+   in the functional semantics for statement, 'k' denotes the execution 
+   steps, whenever it reaches 0, an untermination state is returned;
+   otherwise, it returns either a normal state, or a run time error 
+   or an abnormal state; run time checks (for example, division by 
+   zero check) are encoded inside the functional semantics;
+*)
+Function f_eval_stmt k (s: stack) (c: statement) {struct k}: Return stack := 
+  match k with
+  | 0 => Unterminated
+  | S k' => 
+    match c with
+    | S_Assignment ast_num x e =>
+        match f_eval_expr s e with
+        | Normal v => 
+            match updateG s x (Value v) with
+            | Some s1 => Normal s1
+            | None => Abnormal
+            end
+        | Run_Time_Error => Run_Time_Error
+        | Abnormal => Abnormal
+        | Unterminated => Unterminated
+        end
+    | S_Sequence ast_num c1 c2 =>
+        match f_eval_stmt k' s c1 with
+        | Normal s1 => f_eval_stmt k' s1 c2
+        | Run_Time_Error => Run_Time_Error
+        | Unterminated => Unterminated
+        | Abnormal => Abnormal
+        end
+    | S_If ast_num b c =>
+        match f_eval_expr s b with
+        | Normal (Bool true) => f_eval_stmt k' s c
+        | Normal (Bool false) => Normal s
+        | Run_Time_Error => Run_Time_Error
+        | Unterminated => Unterminated
+        | _ => Abnormal
+        end
+    | S_While_Loop ast_num b c => 
+        match f_eval_expr s b with
+        | Normal (Bool true) => 
+            match f_eval_stmt k' s c with
+            | Normal s1 => f_eval_stmt k' s1 (S_While_Loop ast_num b c)
+            | Run_Time_Error => Run_Time_Error
+            | Unterminated => Unterminated
+            | Abnormal => Abnormal
+            end
+        | Normal (Bool false) => Normal s
+        | Run_Time_Error => Run_Time_Error
+        | Unterminated => Unterminated
+        | _ => Abnormal
+        end
+    | S_ProcCall ast_num pbname lexp =>
+      match fetchG pbname s with
+        | Some (Procedure pb) => 
+          match copy_in s (procedure_parameter_profile pb) lexp with
+            | Normal prefx => 
+              match f_eval_decl s prefx (procedure_declarative_part pb) with
+                | Normal s2 =>
+                  match f_eval_stmt k' (s2::s) (procedure_statements pb) with
+                    | Normal (frame::s') =>
+                      match split1 _ (List.length frame - List.length prefx) frame with
+                        | Some (slocal,prefx') =>
+                          (copy_out prefx' (procedure_parameter_profile pb) lexp s')
+                        | None => Abnormal (* erronous store size *)
+                      end
+                    | Run_Time_Error => Run_Time_Error
+                    | _ => Abnormal (* erronous stack size or abnormal result *)
+                  end
+                | Run_Time_Error => Run_Time_Error
+                | _ => Abnormal
+              end
+            (* left and right are not of the same type (return_state
+               store) and (return_state stack) *)
+            | Run_Time_Error => Run_Time_Error
+            | Abnormal => Abnormal
+            | Unterminated => Unterminated
+          end
+        | _ => (* None or non-procedure *) Abnormal
+      end
+    end
+  end.
+
+
+(** basic lemmas *)
+(** expression semantic is deterministic. *)
+
+Lemma eval_expr_unique: forall s e v1 v2,
+    eval_expr s e v1 ->
+    eval_expr s e v2 ->
+    v1 = v2.
+Proof.
+  intros s e v1 v2 H.
+  revert v2.
+  induction H;intros v' h;try now (inversion h;clear h;subst;try auto).
+  - (inversion h;clear h;subst;try auto).
+    rewrite H in H4.
+    injection H4.
+    intros H0.
+    subst.
+    auto.
+
+  - (inversion h;clear h;subst;try auto).
+    apply IHeval_expr in H5.
+    discriminate.
+    
+  - (inversion h;clear h;subst;try auto).
+    apply IHeval_expr2 in H8.
+    discriminate.
+
+  - (inversion h;clear h;subst;try auto).
+    apply f_do_check_complete in H10.
+    apply f_do_check_complete in H1.
+    apply IHeval_expr2 in H9.
+    apply IHeval_expr1 in H7.
+    injection H7.
+    injection H9.
+    intros; subst.
+    rewrite H10 in H1.
+    discriminate.
+
+  - (inversion h;clear h;subst;try auto).
+    + apply IHeval_expr1 in H9.
+      discriminate.
+    + apply IHeval_expr2 in H10.
+      discriminate.
+
+    + apply f_do_check_complete in H11.
+      apply f_do_check_complete in H1.
+      apply IHeval_expr1 in H9.
+      apply IHeval_expr2 in H10.
+      injection H9.
+      injection H10.
+      intros; subst.
+      rewrite H11 in H1.
+      discriminate.
+
+    + apply IHeval_expr1 in H8.
+      apply IHeval_expr2 in H10.
+      injection H8.
+      injection H10.
+      intros ;subst.
+      rewrite (eval_bin_unique _ _ _ _ _ H12 H2) .
+      reflexivity.
+    
+  - (inversion h;clear h;subst;try auto).
+    apply IHeval_expr in H5.
+    discriminate.
+  - (inversion h;clear h;subst;try auto).
+    + apply IHeval_expr in H6.
+      discriminate.
+    + apply IHeval_expr in H6.
+      injection H6.
+      intros ;subst.
+      rewrite (eval_unary_unique _ _ _ _ H7 H0) .
+      reflexivity.
+Qed.    
+
+
+(** 
+    for any expression e evaluated under the state s, if it can be 
+    evaluated to a value v with respect to the relational semantics 
+    eval_expr, then the result value v should be either a normal 
+    value or a run time error;
+*)
+Lemma eval_expr_state : forall s e v,
+        eval_expr s e v -> (* v should be either a normal value or a run time error *)
+            (exists v0, v = Normal v0) \/ v = Run_Time_Error.
+Proof.
+    intros s e v h.
+    induction h;
+    try match goal with
+    | [ |- (exists v, Normal ?v1 = Normal v) \/ _ ]
+      => left; exists v1; reflexivity
+    | [ |- context [ _ \/ ?A = ?A ] ] => right; reflexivity
+    end; auto.
+Qed.
+
+(** 
+    for any statement c starting from the initial state s, if it 
+    terminates in a state s' with respect to the relational semantics 
+    eval_stmt, then the result state s' should be either a normal 
+    state or a run time error. In relational semantics eval_stmt, 
+    all statements that can go abnormal are excluded;
+*)
+Lemma eval_stmt_state : forall s c s',
+        eval_stmt s c s' -> (* s' is either a normal state or a run time error *)
+            (exists v, s' = Normal v) \/ s' = Run_Time_Error.
+Proof.
+    intros s c s' h.
+    induction h;
+    try match goal with
+    | [ |- (exists v, Normal ?v1 = Normal v) \/ _ ] => left; exists v1; reflexivity
+    | [ |- context [ _ \/ ?A = ?A ] ] => right; reflexivity
+    end; auto.
+Qed.
+
+(** * Bisimulation Between Relational And Functional Semantics *)
+
+(** bisimulation proof between f_eval_binexpr and eval_binexpr:
+    - f_eval_bin_expr_correct
+    - f_eval_bin_expr_complete
+*)
+Lemma f_eval_bin_expr_correct: forall op v1 v2 v,
+    f_eval_bin_expr op v1 v2 = Normal v ->
+    eval_bin_expr op v1 v2 v.
+Proof.
+    intros op v1 v2 v h1.
+    destruct op;
+    match goal with 
+    |[|- eval_bin_expr Divide _ _ _] => idtac
+    |[|- eval_bin_expr ?op _ _ _] =>
+        destruct v1, v2;
+        simpl in h1; inversion h1; subst;
+        constructor; auto
+    end.
+    destruct v1, v2; simpl in h1; inversion h1.
+    constructor.
+    remember (Zeq_bool n0 0) as x.
+    reflexivity.
+Qed.
+
+Lemma f_eval_bin_expr_complete: forall op v1 v2 v,
+    eval_bin_expr op v1 v2 v ->
+    f_eval_bin_expr op v1 v2 = Normal v.
+Proof.
+    intros op v1 v2 v h1.
+    induction h1;
+    rewrite <- H;
+    simpl; auto.
+Qed.
+
+(** bisimulation proof between f_eval_unaryexpr and eval_unaryexpr: 
+    - f_eval_unary_expr_correct
+    - f_eval_unary_expr_complete
+*)
+Lemma f_eval_unary_expr_correct: forall op v v',
+    f_eval_unary_expr op v = Normal v' ->
+    eval_unary_expr op v v'.
+Proof.
+    intros.
+    destruct op; simpl in H.
+    - destruct v; inversion H; subst.
+      constructor; auto.
+    - destruct v;destruct v';simpl in *;try discriminate.
+      injection H.
+      intro.
+      subst.
+      constructor 2.      
+Qed.
+
+Lemma f_eval_unary_expr_complete: forall op v v',
+    eval_unary_expr op v v' ->
+    f_eval_unary_expr op v = Normal v'.
+Proof.
+  intros op v v' h1.
+  induction h1;simpl;subst;auto.
+Qed.
+
+(** ** Bisimulation between f_eval_expr and eval_expr for expression Semantics *)
+(** a help lemma to prove the theorem: f_eval_expr_correct *)
+Lemma f_eval_expr_correct1 : forall s e v,
+                        f_eval_expr s e = Normal v ->
+                            eval_expr s e (Normal v).
+Proof.
+    intros s e.
+    functional induction (f_eval_expr s e);
+    intros v0 h1;
+    try inversion h1; subst.
+  - constructor;
+    reflexivity.
+  - constructor;
+    assumption.
+  - specialize (IHr _ e3).
+    specialize (IHr0 _ e4).
+    rewrite H0.
+    econstructor.
+    exact IHr. exact IHr0.
+    + apply f_do_check_correct.
+      auto.
+    + apply f_eval_bin_expr_correct; 
+      auto.
+  - specialize (IHr _ e2).
+    rewrite h1.
+    econstructor. 
+    exact IHr.
+    destruct op. 
+    + simpl in h1. 
+      destruct v; inversion h1; subst.
+      constructor; auto.
+    + simpl in h1. 
+      destruct v; inversion h1; subst.
+      constructor; auto.
+Qed.
+
+(** another help lemma to prove the theorem: f_eval_expr_correct *)
+Lemma f_eval_expr_correct2 : forall s e,
+                        f_eval_expr s e = Run_Time_Error ->
+                            eval_expr s e Run_Time_Error.
+Proof.
+    intros s e.
+    functional induction (f_eval_expr s e);
+    intros h; try inversion h.
+  - destruct op, v1, v2;
+    simpl in h; inversion h.
+  - specialize (f_eval_expr_correct1 _ _ _ e3); intros hz1.
+    specialize (f_eval_expr_correct1 _ _ _ e4); intros hz2.
+    eapply eval_E_Binary_Operation3.
+    apply hz1. apply hz2.
+    apply f_do_check_correct; auto.
+  - specialize (f_eval_expr_correct1 _ _ _ e3); intros hz1.
+    specialize (IHr0 e4).
+    eapply eval_E_Binary_Operation2; auto.
+    exact hz1.
+  - specialize (IHr e3).
+    constructor; assumption.
+  - destruct op;
+    destruct v; inversion h. 
+  - specialize (IHr e2).
+    constructor; assumption.
+Qed.
+
+(** *** f_eval_expr_correct *)
+(** 
+    for an expression e evaluated under the state s with respect to
+    the functional semantics f_eval_expr, whenever it returns a 
+    normal value v or terminates in a run time error, 
+    the relation between s, e and evaluation result should also be 
+    satisfied with respect to the relational semantics 'eval_expr';
+*)
+Theorem f_eval_expr_correct : forall s e v,
+                        (f_eval_expr s e = Normal v ->
+                            eval_expr s e (Normal v)) /\
+                        (f_eval_expr s e = Run_Time_Error ->
+                            eval_expr s e Run_Time_Error).
+Proof.
+    split.
+  - apply f_eval_expr_correct1.
+  - apply f_eval_expr_correct2.
+Qed.
+
+
+(** *** f_eval_expr_complete *)
+(** 
+   for any expression e, if it can be evaluated to a value v under
+   state s with respect to the relational semantics 'eval_expr', 
+   then when we evalute e under the same state s in functional
+   semantics 'f_eval_expr', it should return the same result v;
+*)
+Theorem f_eval_expr_complete : forall e s v,  
+                        eval_expr e s v -> 
+                            (f_eval_expr e s) = v.
+Proof.
+    intros e s v h.
+    induction h; simpl; intros;
+    repeat match goal with
+    | h: fetchG _ _ = _  |- _ => progress rewrite h
+    | h: f_eval_expr _ _ = _ |- _ => progress rewrite h
+    end;auto.
+  - rewrite H; reflexivity.
+  - specialize (f_do_check_complete _ _ _ _ H); intros hz1.
+    rewrite hz1.
+    reflexivity.
+  - destruct v1; destruct v2;
+    destruct op;
+    inversion H0; subst; simpl; auto.
+    + (* overflow check for Plus *)
+      inversion H; subst.
+      rewrite H3; auto.
+      unfold not in H2; intuition.
+    + (* overflow check for Minus *)
+      inversion H; subst.
+      rewrite H3; auto.
+      unfold not in H2; intuition.
+    + (* overflow check for Multiply *)
+      inversion H; subst.
+      rewrite H3; auto.
+      unfold not in H2; intuition.
+    + (* both division by zero check and overflow check *)
+      inversion H; subst.
+      rewrite H3; auto.
+      rm_false_hyp.
+  - destruct op.
+    + inversion H; subst.
+      auto.
+    + inversion H; subst.
+      auto.
+Qed.
+
+
+
+Ltac discriminate2 :=
+  let rewd HH HH' y z :=
+      match y with 
+        | z => fail 
+        | _ => rewrite HH in HH';discriminate
+  end in
+    match goal with
+      | HH: ?x = ?y , HH': ?x = ?z |- _ => rewd HH HH' y z
+      | HH: ?x = ?y , HH': ?z = ?x |- _ => rewd HH HH' y z 
+      | HH: ?y = ?x , HH': ?x = ?z |- _ => symmetry in HH; rewd HH HH' y z
+      | HH: ?y = ?x , HH': ?z = ?x |- _ => symmetry in HH; rewd HH HH' y z
+    end.
+
+
+
+Ltac apply_inv :=
+  try discriminate; try discriminate2;
+  match goal with
+    | H:Normal _ = Normal _ |- _ => inversion H;clear H;subst 
+    | H:update _ _ (Value _) = _ |- _ => rewrite H
+    | H:updateG _ _ (Value _) = _ |- _ => rewrite H
+    | H:f_eval_stmt _ _ _ = _ |- _ => rewrite H
+    | H:f_eval_expr _ _ = _ |- _ => rewrite H
+    | H:f_eval_decl _ _ _ = _ |- _ => rewrite H
+    | H:copy_out _ _ _ _ = _ |- _ => rewrite H
+    | H:copy_in _ _ _ = _ |- _ => rewrite H
+    | H:fetch _ _ = _ |- _ => rewrite H
+    | H:fetchG _ _ = _ |- _ => rewrite H
+    | H:split2 _ _ _ = _ |- _ => rewrite H
+    | H:split1 _ _ _ = _ |- _ => rewrite H
+  end;subst;simpl;auto.
+
+Ltac invle := match goal with
+    | H: (S _ <= _)%nat |- _ => (inversion H; clear H; subst; simpl)
+  end.
+
+(** a help lemma to prove the theorem: 'f_eval_stmt_complete',
+    it means that: for any statement c, starting from initial state s, 
+    if it terminates in a normal state s' within k execution steps, 
+    then for any k' greater and equal than k, it should also terminate 
+    in the same state s';
+*)
+Lemma f_eval_stmt_fixpoint: forall k s c s', 
+        f_eval_stmt k s c = Normal s' ->
+        forall k':nat, (k <= k')%nat -> 
+            f_eval_stmt k' s c = Normal s'.
+Proof.
+    intros k s c.
+    functional induction (f_eval_stmt k s c); simpl; intros; subst; simpl; auto;
+    repeat progress apply_inv.
+  - invle; repeat apply_inv.
+  - invle.
+    + repeat apply_inv.
+    + rewrite (IHr _ e1);auto with arith.
+  - invle; repeat apply_inv. rewrite (IHr _ H);auto with arith.
+  - invle; repeat apply_inv.
+  - invle; repeat apply_inv. rewrite (IHr _ e2); auto with arith.
+  - invle; repeat apply_inv.
+  - invle; repeat apply_inv.
+    + rewrite (IHr _ e4).
+      repeat apply_inv.
+      auto with arith.
+Qed.
+
+(** another help lemma to prove the theorem: 'f_eval_stmt_complete' *)
+Lemma f_eval_stmt_fixpoint_E: forall k s p, 
+        f_eval_stmt k s p = Run_Time_Error ->
+        forall k':nat, (k <= k')%nat -> 
+            f_eval_stmt k' s p = Run_Time_Error.
+Proof.
+    intros k s p.
+    functional induction (f_eval_stmt k s p); simpl; intros; subst; simpl; auto;
+    repeat progress apply_inv. 
+  - invle;
+    apply_inv.
+  - invle;
+    repeat apply_inv.
+    rewrite (f_eval_stmt_fixpoint _ _ _ _ e1); auto with arith.
+  - invle;
+    repeat apply_inv.
+    specialize (IHr e1). 
+    rewrite IHr; auto with arith. 
+  - invle; 
+    repeat apply_inv.
+    rewrite IHr; auto with arith.
+  - invle;
+    repeat apply_inv.
+  - invle; 
+    repeat apply_inv. 
+    rewrite (f_eval_stmt_fixpoint _ _ _ _ e2); auto with arith.
+  - invle; 
+    repeat apply_inv.
+    rewrite (IHr e2); auto with arith.    
+  - invle; 
+    repeat apply_inv.   
+  - invle; repeat apply_inv.
+    rewrite (f_eval_stmt_fixpoint _ _ _ _ e4); auto with arith.
+    rewrite e5.
+    assumption.
+  - invle; repeat apply_inv.
+    rewrite  (IHr e4 m);auto with arith.
+  - clear H.
+    invle; repeat apply_inv.
+  - invle; repeat apply_inv.
+Qed.
+
+
+Ltac destrIH :=
+  repeat progress (match goal with
+                     | h: ex _ |- _  =>
+                       let k := fresh "k" in
+                       let hk1 := fresh "hk" in
+                       destruct (h) as [k hk1];try assumption
+                   end).
+
+Ltac kgreater :=
+  repeat
+    match goal with
+      | h:f_eval_stmt ?k ?s ?p = Normal ?s' |- context [f_eval_stmt (?k + _) ?s ?p] =>
+        rewrite (@f_eval_stmt_fixpoint _ _ _ _ h);auto with arith
+      | h:f_eval_stmt ?k ?s ?p = Normal ?s' |- context [f_eval_stmt (_ + ?k) ?s ?p] =>
+        rewrite (@f_eval_stmt_fixpoint _ _ _ _ h);auto with arith
+      | h:f_eval_stmt ?k ?s ?p = Run_Time_Error |- context [f_eval_stmt (?k + _) ?s ?p] =>
+        rewrite (@f_eval_stmt_fixpoint_E _ _ _ h);auto with arith
+      | h:f_eval_stmt ?k ?s ?p = Run_Time_Error |- context [f_eval_stmt (_ + ?k) ?s ?p] =>
+        rewrite (@f_eval_stmt_fixpoint_E _ _ _ h);auto with arith
+         end.
+
+
+Ltac rm_eval_expr :=
+  match goal with 
+    | [ h: eval_expr ?s ?b ?X, h': f_eval_expr ?s ?b = ?X |- _ ] => clear h
+    | [ h: eval_expr ?s ?b ?X, h': ?X = f_eval_expr ?s ?b |- _ ] => clear h; symmetry in h'
+    | [ h: eval_expr ?s ?b ?X |- _ ] => apply f_eval_expr_complete in h
+  end; auto.
+
+
+Ltac rewinv h h' := rewrite h in h'; inversion h'; try clear h' ; subst.
+
+(* This tactic is a generalization of inversion. We first rewrite with
+   some equality about function f first, and then do inversion on the
+   rewritten hypothesis. The tactic removes the inversed hypothesis at
+   the end so this *should* never loop. *)
+Ltac inversion2 f :=
+  match goal with
+    | H: f ?X = _ , H': context [f ?X] |- _ => rewinv H H'
+    | H: f ?X ?Y = _ , H': context [ f ?X ?Y ] |- _ => rewinv H H'
+    | H: f ?X ?Y ?Z = _ , H': context [ f ?X ?Y ?Z ] |- _ => rewinv H H'
+    | H: f ?X ?Y ?Z ?U = _ , H': context [ f ?X ?Y ?Z ?U ] |- _ => rewinv H H'
+    | H: f ?X ?Y ?Z ?U ?V = _ , H': context [ f ?X ?Y ?Z ?U ?V ] |- _ => rewinv H H'
+    | H: f ?X ?Y ?Z ?U ?V ?W = _ , H': context [ f ?X ?Y ?Z ?U ?V ?W ] |- _ => rewinv H H'
+    (* Same with a left to right equality *)
+    | H: _ = f ?X , H': context [f ?X] |- _ => rewinv H H'
+    | H: _ = f ?X ?Y , H': context [ f ?X ?Y ] |- _ => rewinv H H'
+    | H: _ = f ?X ?Y ?Z , H': context [ f ?X ?Y ?Z ] |- _ => rewinv H H'
+    | H: _ = f ?X ?Y ?Z ?U , H': context [ f ?X ?Y ?Z ?U ] |- _ => rewinv H H'
+    | H: _ = f ?X ?Y ?Z ?U ?V , H': context [ f ?X ?Y ?Z ?U ?V ] |- _ => rewinv H H'
+    | H: _ = f ?X ?Y ?Z ?U ?V ?W , H': context [ f ?X ?Y ?Z ?U ?V ?W ] |- _ => rewinv H H'
+  end ; auto.
+
+
+
+Lemma copy_in_correct:
+  forall s prm lexp prefx,
+    copy_in s prm lexp = (Normal prefx) <->  Copy_in s prm lexp (Normal prefx).
+Proof.
+  intros s prm lexp.
+  functional induction copy_in s prm lexp;intros;split;simpl in *;intro heq
+  ; try (inversion heq;subst;clear heq)
+  ; repeat rm_eval_expr
+  ; try repeat progress match goal with (* Rewrite induction hyp if you can *)
+                          | H: (forall _, ?X = _ <-> _)  |- _ =>
+                            rewrite <- H in *
+                        end
+  ; try (now repeat progress
+             first [ discriminate2
+                   | inversion2 copy_in;auto
+                   | inversion2 f_eval_expr;auto ]).
+  - inversion_is_var e2.
+    econstructor 2.
+    + apply IHr;auto.
+    + assumption.
+
+  - apply Copy_in_cons_in.
+    + apply IHr.
+      assumption.
+    + assumption.
+    + apply f_eval_expr_correct1.
+      assumption.
+  - constructor 1.
+Qed.
+
+
+
+Lemma copy_in_correct2:
+  forall s prm lexp,
+    copy_in s prm lexp = Run_Time_Error <->  Copy_in s prm lexp Run_Time_Error.
+Proof.
+  intros s prm lexp.
+  functional induction copy_in s prm lexp;intros;split;simpl in *;intro heq
+  ; try (inversion heq;subst;clear heq)
+  ; repeat try rm_eval_expr
+  ; try repeat progress (* Rewrite with induction hyp as much as we can *)
+        match goal with
+          | H: (?X = _ <-> _)  |- _ =>
+            rewrite <- H in *
+        end
+  ; try (now repeat progress
+             first [ discriminate2
+                   | inversion2 copy_in;auto
+                   | inversion2 f_eval_expr;auto ]).
+  - inversion_is_var e2.
+    rewrite H0.
+    econstructor;auto.
+    rewrite <- IHr.
+    assumption.
+  - rewrite H0.
+    apply Copy_in_cons_in_rte2 with (v:=v');auto.
+    + rewrite <- IHr.
+      assumption.
+    + apply f_eval_expr_correct1.
+      assumption.
+  - apply Copy_in_cons_in_rte1;auto.
+    apply f_eval_expr_correct2.
+    assumption.
+Qed.
+
+Lemma Copy_out_stack_eq_length :
+  forall prefx prm lexp s s',
+    Copy_out prefx prm lexp s s'
+    -> stack_eq_length s s'.
+Proof.
+  intros prefx prm lexp s s' H.
+  induction H;auto.
+  - apply stack_eq_length_refl.
+    reflexivity.
+  - apply updateG_stack_eq_length in H2.
+    apply stack_eq_length_trans with σ';auto.
+Qed.
+
+Lemma Copy_out_length :
+  forall prefx prm lexp s s',
+    Copy_out prefx prm lexp s s'
+    -> List.length s = List.length s'.
+Proof.
+  intros prefx prm lexp s s' H.
+  induction H;auto.
+  transitivity (List.length σ');auto.
+  apply updateG_length in H2.
+  assumption.
+Qed.
+
+
+
+Lemma copy_out_no_rte:
+  forall prefx lprm lexp s,
+    ~ copy_out prefx lprm lexp s = Run_Time_Error.
+Proof.
+  intros prefx lprm lexp s.
+  functional induction copy_out prefx lprm lexp s;try assumption;try discriminate.
+Qed.
+
+
+Lemma copy_out_correct:
+  forall prefx s (prm:list parameter_specification) lexp x,
+    copy_out prefx prm lexp s = Normal x <-> Copy_out prefx prm lexp s x.
+Proof.
+  intros prefx s prm lexp.
+  functional induction copy_out prefx prm lexp s;intros;split;simpl in *;intro heq
+  ; try (now (inversion heq;subst;clear heq);auto;try now (econstructor;eauto)).
+  - apply Copy_out_cons_out with (σ':=s') (v:=v)(id:=parameter_name prm);auto.
+    apply IHr.
+    assumption.
+  - inversion heq;subst.
+    + inversion2 fetch.
+      apply IHr.
+      inversion2 updateG.
+    + rewrite e2 in *.
+      discriminate.
+  - inversion heq;clear heq;subst.
+    + inversion2 fetch.
+      rewrite H10 in *.
+      discriminate e5.
+    + rewrite e2 in *.
+      discriminate.
+  - inversion heq;clear heq;subst.
+    + inversion2 fetch.
+    + rewrite e2 in *.
+      discriminate.
+  - inversion heq;subst;try contradiction.
+    rewrite e2 in *.
+    discriminate.
+  - constructor 3;auto.
+    apply IHr.
+    assumption.
+  - inversion heq;subst;try contradiction.
+    + rewrite e2 in *.
+      discriminate.
+    + apply IHr.
+      assumption.
+  - inversion heq;subst;try contradiction.
+    + rewrite H3 in *;contradiction.
+    + rewrite H6 in *;contradiction.
+Qed.
+
+
+
+
+
+Lemma eval_decl_store_length:
+  forall s sto s' decl,
+    eval_decl s sto decl s'
+    -> forall st, s' = Normal st
+                  -> exists prfx, st = prfx ++ sto.
+Proof.
+  intros s sto s' decl h.
+  induction h;intros st heq;inversion heq;clear heq;subst.
+  - exists ((object_name d, Value v)::nil).
+    simpl.
+    reflexivity.
+  - exists ((object_name d, Undefined)::nil);simpl.
+    reflexivity.
+  - destruct (IHh2 st).
+    { reflexivity. }
+    destruct (IHh1 s').
+    { reflexivity. }
+    subst.
+    exists (x ++ x0).
+    apply app_assoc.
+  - exists ((procedure_name pbody, Procedure pbody)::nil);simpl.
+    reflexivity.
+Qed.
+
+
+
+Lemma eval_stmt_store_length:
+  forall s s' stm,    
+    eval_stmt s stm s'
+    -> forall st, s' = Normal st
+                  -> stack_eq_length s st.
+Proof.
+  intros s s' stm H.
+  induction H;intros st heq;inversion heq;clear heq; subst;auto.
+  - apply updateG_stack_eq_length in H0.
+    assumption.
+  - apply stack_eq_length_trans with s1.
+    + apply IHeval_stmt1.
+      reflexivity.
+    + apply IHeval_stmt2.
+      reflexivity.
+  - apply stack_eq_length_refl.
+    reflexivity.
+  - apply stack_eq_length_trans with s1.
+    + apply IHeval_stmt1.
+      reflexivity.
+    + apply IHeval_stmt2.
+      reflexivity.
+  - apply stack_eq_length_refl.
+    reflexivity.
+  - 
+    specialize (IHeval_stmt ((slocal ++ prefix') :: s') eq_refl).
+    inversion IHeval_stmt.
+    clear IHeval_stmt.
+    subst.
+    apply stack_eq_length_trans with s'.
+    + assumption.
+    + apply Copy_out_stack_eq_length in H5.
+      assumption.
+Qed.
+
+Lemma f_eval_decl_correct :
+  forall s sto d s',
+    f_eval_decl s sto d = Normal s' ->
+    eval_decl s sto d (Normal s').
+Proof.
+  intros s sto d.
+  functional induction f_eval_decl s sto d;simpl;intros;try discriminate
+  ; try match goal with
+        | H: Normal _ = Normal _ |- _ =>
+          inversion H;subst;clear H
+      end;try now( (econstructor;eauto;try apply f_eval_expr_correct1;auto)).
+  - rewrite H in y.
+    contradiction.
+Qed.
+
+Lemma f_eval_decl_correct2 :
+  forall s sto d,
+    f_eval_decl s sto d = Run_Time_Error ->
+    eval_decl s sto d Run_Time_Error.
+Proof.
+  intros s sto d.
+  functional induction f_eval_decl s sto d;simpl;intros;try discriminate;
+  try match goal with
+        | H: Normal _ = Run_Time_Error |- _ =>
+          inversion H;subst;clear H
+      end;try now( (econstructor;eauto);try apply f_eval_expr_correct2;auto).
+  
+  eapply eval_decl_Seq_err2 with s';auto.
+  apply f_eval_decl_correct.
+  assumption.
+Qed.
+
+Ltac invclear H := inversion H; clear H; subst.
+
+Ltac use_determinism :=
+  match goal with
+    | H : ?X = ?X |- _ => clear H
+    | H: None = ?y, H': ?y = Some ?z |- _ => rewrite H' in H; invclear H
+    | H: Some ?z = ?y, H': ?y = None |- _ => rewrite H' in H; invclear H
+    | H: Some ?x = ?y, H': ?y = Some ?z |- _ => rewrite H' in H; inversion H;clear H;subst
+    | H : eval_expr ?s ?e ?X,
+          H': f_eval_expr ?s ?e = ?Y |- _ => rewrite (f_eval_expr_complete s e X H) in H'
+    | H:  eval_expr ?s ?e ?X,
+          H': eval_expr ?s ?e ?Y |- _ => apply (f_eval_expr_complete s e X) in H
+         ;apply (f_eval_expr_complete s e) in H'
+    | H : f_eval_expr ?s ?e = ?X,
+          H': f_eval_expr ?s ?e = ?Y |- _ => rewrite H in H'; invclear H'
+    | H : (Normal ?v) = (Normal ?v') |- _ => invclear H
+  end.
+
+Ltac crush := repeat progress use_determinism;try reflexivity;try discriminate.
+
+Lemma f_eval_decl_complete :
+  forall d sto s s',
+    eval_decl s sto d s' ->
+    f_eval_decl s sto d = s'.
+Proof.
+  intros d sto s.
+  functional induction f_eval_decl s sto d;simpl;intros;try discriminate;crush;
+  try now (invclear H;crush).
+  - invclear H
+    ; try match goal with
+            | H: eval_decl _ _ dcl1 _ |- _ => rename H into hed1
+          end
+    ; try match goal with
+            | H: eval_decl _ _ dcl2 _ |- _ => rename H into hed2
+          end. 
+    + apply IHr in hed1.
+      rewrite e0 in hed1.
+      inversion hed1.
+      subst.
+      apply IHr0 in hed2.
+      assumption.
+    + apply IHr in hed1.
+      rewrite e0 in hed1.
+      inversion hed1.
+    + apply IHr in hed1.
+      rewrite e0 in hed1.
+      inversion hed1.
+      subst.
+      apply IHr0 in hed2.
+      assumption.
+  - invclear H
+    ; try match goal with
+            | H: eval_decl _ _ dcl1 _ |- _ => rename H into hed1
+          end
+    ; try match goal with
+            | H: eval_decl _ _ dcl2 _ |- _ => rename H into hed2
+          end.
+    + apply IHr in hed1.
+      rewrite hed1 in y.
+      contradiction.
+    + apply IHr in hed1.
+      assumption.
+    + apply IHr in hed1.
+      rewrite hed1 in y.
+      contradiction.
+Qed.
+
+
+(** ** Bisimulation between f_eval_stmt and eval_stmt for statement semantics *)
+
+
+Ltac rm_f_eval_expr :=
+  match goal with 
+    | [ h: f_eval_expr ?s ?b = Run_Time_Error |- _ ] => 
+      specialize (f_eval_expr_correct2 _ _ h); intros hz1
+    | [ h: f_eval_expr ?s ?b = Normal ?v |- _ ] => 
+      specialize (f_eval_expr_correct1 _ _ _ h); intros hz1   
+  end; auto.
+
+
+
+(** a help lemma to prove the theorem: 'f_eval_stmt_complete' *)
+Lemma f_eval_stmt_correct1 : forall k s p s',
+        f_eval_stmt k s p = Normal s' ->
+          eval_stmt s p (Normal s').
+Proof.
+    intros k s p.
+    functional induction (f_eval_stmt k s p);
+    intros; try inversion H; subst.
+  - (* S_Assignment *)
+    econstructor.
+    rm_f_eval_expr.
+    apply hz1.
+    assumption.
+  - (* S_Sequence *)
+    specialize (IHr _ e1).
+    specialize (IHr0 _ H).
+    econstructor.
+    apply IHr.
+    apply_inv.
+  - (* S_If_True *)
+    specialize (IHr _ H).
+    econstructor.
+    rm_f_eval_expr. 
+    apply_inv.
+  - (* S_If_False *)
+    eapply eval_S_If_False.
+    rm_f_eval_expr.
+  - (* S_While_Loop_True *)
+    specialize (IHr _ e2).
+    specialize (IHr0 _ H).
+    econstructor.
+    rm_f_eval_expr.
+    apply IHr. 
+    apply_inv.
+  - (* S_While_Loop_False *)
+    eapply eval_S_While_Loop_False.
+    rm_f_eval_expr.
+  - (* S_ProcCall *)
+    clear H.
+    (* cleaning by going to inductive defs *)
+    apply split1_correct in e5.
+    destruct e5 as [hsplit1 hsplit2].
+    rewrite H1.
+    subst.
+    apply f_eval_decl_correct in e3.    
+    apply IHr in e4.
+    apply copy_in_correct in e2.
+    apply copy_out_correct in H1.
+    (* ******* *)
+    eapply eval_S_Proc with (s':=s') (prefix':=prefx')(prefix:=prefx)(slocal:=slocal);eauto.
+    eapply eval_decl_store_length with (st:=s2) in e3;auto.
+    destruct e3 as [slocal' ?]. subst.
+    apply eval_stmt_store_length with (st:=((slocal ++ prefx') :: s')) in e4;auto.
+    inversion e4. clear e4. subst.
+    rewrite <- H5 in hsplit1.
+    setoid_rewrite app_length in H5.
+    setoid_rewrite app_length in hsplit1.
+    omega.
+Qed.
+
+
+Ltac rm_f_eval_stmt :=
+    match goal with 
+    | [ h: f_eval_stmt ?k ?s ?c = Normal ?s1 |- _ ] => 
+        specialize (f_eval_stmt_correct1 _ _ _ _ h); intros hz1
+    end; auto.
+
+(** a help lemma to prove the theorem: 'f_eval_stmt_complete' *)
+Lemma f_eval_stmt_correct2 : forall k s p,
+        f_eval_stmt k s p = Run_Time_Error ->
+          eval_stmt s p Run_Time_Error.
+Proof.
+    intros k s p.
+    functional induction (f_eval_stmt k s p);
+      intros H ; try inversion H;  subst.
+  - (* S_Assignment *)
+    econstructor.
+    rm_f_eval_expr.
+  - (* S_Sequence*)
+    specialize (IHr0 H).
+    econstructor.
+    rm_f_eval_stmt.
+    apply hz1.
+    apply_inv.
+  - specialize (IHr e1).
+    econstructor.
+    assumption.    
+  - (* C_If *)
+    specialize (IHr H).
+    econstructor.
+    rm_f_eval_expr.
+    apply_inv.
+  - econstructor.
+    specialize (f_eval_expr_correct2 _ _ e1); intros hz1. 
+    assumption.
+  - (* S_While_Loop *)
+    specialize (IHr0 H).
+    econstructor.
+    rm_f_eval_expr.
+    rm_f_eval_stmt.
+    apply hz1.
+    apply_inv.
+  - constructor 9.
+    rm_f_eval_expr.
+    specialize (IHr e2); assumption.    
+  - econstructor.
+    rm_f_eval_expr.
+  - elim (copy_out_no_rte _ _ _ _ H1).
+  - apply eval_S_Proc_rtebody with (prefix:=prefx) (s2:=s2) (pb:=pb);auto. 
+    + apply copy_in_correct.
+      assumption.
+    + apply f_eval_decl_correct.
+      assumption.
+  - eapply eval_S_Proc_rtedecl with (prefix:=prefx);eauto.
+    + apply copy_in_correct.
+      assumption.
+    + eapply f_eval_decl_correct2.
+      assumption.
+  - eapply eval_S_Proc_rteargs with pb;auto.
+    apply copy_in_correct2.
+    assumption.
+Qed.
+    
+    
+
+Ltac rm_f_eval :=
+    match goal with 
+    | [ h: f_eval_expr ?s ?b = Run_Time_Error |- _ ] => specialize (f_eval_expr_correct2 _ _ h); intros hz1
+    | [ h: f_eval_expr ?s ?b = Normal ?v |- _ ] => specialize (f_eval_expr_correct1 _ _ _ h); intros hz1   
+    | [ h: f_eval_stmt ?k ?s ?c = Run_Time_Error |- _ ] => specialize (f_eval_stmt_correct2 _ _ _ h); intros hz1
+    | [ h: f_eval_stmt ?k ?s ?c = Normal ?s1 |- _ ] => specialize (f_eval_stmt_correct1 _ _ _ _ h); intros hz1
+    end; auto.
+
+(** *** f_eval_stmt_correct *)
+(** 
+   for any statement c starting from initial state s, if it returns 
+   a normal state s' or terminates in a run time error within k steps
+   with respect to the functional semantics 'f_eval_stmt', then the 
+   relation between s, c and the resulting state should also be 
+   satisfied with respect to the relational semantics 'eval_stmt';
+*)
+Theorem f_eval_stmt_correct : forall k s c s',
+        (f_eval_stmt k s c = Normal s' ->
+          eval_stmt s c (Normal s')) /\ 
+        (f_eval_stmt k s c = Run_Time_Error ->
+          eval_stmt s c Run_Time_Error).
+Proof.
+    intros.
+    split; intros;
+    rm_f_eval.
+Qed.
+
+(** *** f_eval_stmt_complete *)
+(** 
+   the reverse direction is also satisfied: for any statement c, 
+   whenever it's executed starting from initial state s and return 
+   a new state s' with regard to the relational semantics 'eval_stmt', 
+   then there should exist a constant k that statement c starting from 
+   s will terminate in state s' within k steps with respect to the 
+   functional semantics 'f_eval_stmt';
+*)
+
+Ltac apply_rewrite := 
+    match goal with
+    | h: eval_expr ?s ?e ?s' |- _ => 
+        rewrite (f_eval_expr_complete _ _ _ h)
+    | h: update _ _ _ = _ |- _ => rewrite h
+    | h: updateG _ _ _ = _ |- _ => rewrite h
+    | h: f_eval_stmt _ _ _ = _ |- _ => rewrite h
+    | h: f_eval_expr _ _ = _ |- _ => rewrite h
+    | h: fetch _ _ = _ |- _ => rewrite h
+    | h: fetchG _ _ = _ |- _ => rewrite h
+    | h: copy_in _ _ _ = _ |- _ => rewrite h
+    | h: Copy_in _ _ _ Run_Time_Error |- _ => rewrite <- copy_in_correct2 in h;rewrite h
+    | h: Copy_in _ _ _ (Normal _) |- _ => rewrite <- copy_in_correct in h;rewrite h
+    end; auto.
+
+Theorem f_eval_stmt_complete : forall s c s',
+        eval_stmt s c s' -> (* s' is either a normal state or a run time error *)
+            exists k, f_eval_stmt k s c = s'.
+Proof. 
+  intros s c s' H;
+  induction H;
+  try match goal with
+  [ h: eval_expr ?s ?e Run_Time_Error |- exists k, _ = Run_Time_Error] => 
+          exists 1%nat; simpl;
+          rewrite (f_eval_expr_complete _ _ _ h);
+          reflexivity
+  end.
+  (* 1. S_Assignment *)
+  - exists 1%nat; simpl.
+    repeat apply_rewrite.
+  (* 2. S_Sequence *)
+  - destrIH.
+    exists (S k); simpl.
+    apply_rewrite.
+  - destrIH.
+    exists (S (k0+k)); simpl.
+    kgreater.
+    specialize (eval_stmt_state _ _ _ H0); intros hz1.
+    destruct hz1 as [hz2 | hz2]; try rm_exists; subst;
+    kgreater.
+  (* 3. S_If *)
+  - destrIH.
+    exists (S k); simpl.
+    apply_rewrite.
+  - exists 1%nat; simpl.
+    apply_rewrite.
+  (* 4. S_While_Loop *)
+  - destrIH.
+    exists (S k); simpl.
+    repeat apply_rewrite.
+  - destrIH.
+    exists (S (k0+k)); simpl.
+    apply_rewrite.
+    kgreater.
+    specialize (eval_stmt_state _ _ _ H1); intros hz1.
+    destruct hz1 as [hz2 | hz2]; try rm_exists; subst;
+    kgreater.
+  - exists 1%nat; simpl.
+    apply_rewrite.
+  - exists 1%nat; simpl.
+    repeat progress apply_rewrite.
+  - exists 1%nat; simpl.
+    subst.
+    repeat apply_rewrite.
+    apply f_eval_decl_complete in H1.
+    rewrite H1.
+    reflexivity.
+  - destruct IHeval_stmt as [k IH].
+    exists (S k).
+    simpl.
+    subst.
+    apply f_eval_decl_complete in H1.
+    repeat apply_rewrite.
+    rewrite H1.
+    apply_rewrite.
+  - destruct IHeval_stmt as [k IH].
+    exists (S k).
+    simpl.
+    subst.
+    repeat apply_rewrite.
+    apply f_eval_decl_complete in H1.
+    rewrite H1.
+    repeat apply_rewrite.
+    repeat setoid_rewrite app_length.
+    rewrite H4.
+    assert (heq:Datatypes.length slocal + Datatypes.length prefix' -
+        Datatypes.length prefix' = Datatypes.length slocal) by omega.
+    rewrite heq.
+    rewrite split1_complete with (l2:=prefix') (l1:=slocal).
+    + apply copy_out_correct.
+      assumption.
+    + reflexivity.
+    + reflexivity.
+Qed.
+
+(**********************************************************************)
+(**********************************************************************)
+
+(** * Subprogram Semantics *)
+
+(** In the current SPARK subset, there is no procedure call, 
+    so right now we only define the semantics for the main procedure.
+    And it can be used to test the tool chain from SPARK source code 
+    to Coq evaluation; Later, we will add the procedure call and 
+    modify the following procedure semantics;
+*)
+
+(** all declared variables in the same procedure should have unique 
+    names; 
+*)
+
+(** relational (eval_decl) and functional (f_eval_decl) semantics for 
+    variable declaration;
+*)
+
+(** for any initial state s, after executing the declaration d, 
+    it either returns a normal state s' or a run time error;
+    (for any variable declaration, if its initialization expression 
+     fails the run time checks, for example division by zero or overflow, 
+     then it returns an exception)
+*)
+
+Lemma eval_decl_state : forall s sto d s',
+        eval_decl s sto d s' -> (* s' is either a normal state or a run time error *)
+            (exists t, s' = Normal t) \/ s' = Run_Time_Error.
+Proof.
+    intros s sto d s' h.
+    induction h;
+    try match goal with
+    | [ |- (exists t, Normal ?t1 = Normal t) \/ _ ] => left; exists t1; reflexivity
+    | [ |- context [ _ \/ ?A = ?A ] ] => right; reflexivity
+    end; auto.
+Qed.
+
+
+(** f_eval_decl completeness and correctness proofs *)
+
+(** bisimulation proof between f_eval_decl and eval_decl: 
+    - f_eval_decl_correct
+    - f_eval_decl_complete
+*)
+
+Lemma f_eval_decl_correct_: forall d s sto s',
+    (f_eval_decl s sto d = (Normal s') -> eval_decl s sto d (Normal s')) /\
+    (f_eval_decl s sto d = Run_Time_Error -> eval_decl s sto d Run_Time_Error).
+Proof.
+    intros d s sto.
+    intros s'.
+    split;intro h.
+    - apply f_eval_decl_correct.
+      assumption.
+    - apply f_eval_decl_correct2.
+      assumption.
+Qed.
+
+
+(* = = = = = = Subprogram Body = = = = = =  *)
+(** relational and functional semantics for procedure body; *)
+(* Is this still needed for global procedures? probably not. *)
+(* main procedure has no argument, so we give the nil store as
+   parameter store *)
+Inductive eval_proc: stack -> procedure_body -> Return stack -> Prop :=
+    | eval_Proc_E: forall f s,
+        eval_decl s nil (procedure_declarative_part f) Run_Time_Error ->
+        eval_proc s f Run_Time_Error
+    | eval_Proc: forall f s1 s2 s3,
+        eval_decl s1 nil (procedure_declarative_part f) (Normal s2) ->
+        eval_stmt (s2::s1) (procedure_statements f) s3 ->
+        eval_proc s1 f s3.
+
+Function f_eval_proc k (s: stack) (f: procedure_body): Return stack :=
+    match (f_eval_decl s nil (procedure_declarative_part f)) with
+    | Normal s' => f_eval_stmt k (s'::s) (procedure_statements f)
+    | Run_Time_Error => Run_Time_Error
+    | Abnormal => Abnormal
+    | Unterminated => Unterminated
+    end.
+
+
+(** ** Main Procedure Evaluation Without Parameters *)
+
+(** relational and functional semantics for main procedure; *)
+
+Inductive eval_subprogram: stack -> subprogram -> Return stack -> Prop :=
+    | eval_Procedure: forall s s' ast_num f,
+        eval_proc s f s' ->
+        eval_subprogram s (Global_Procedure ast_num f) s'.
+
+Function f_eval_subprogram k (s: stack) (f: subprogram): Return stack := 
+    match f with 
+    | Global_Procedure ast_num f' => f_eval_proc k s f'
+    end.
+
+(** ** Bisimulation Between Relational And Functional Semantics For Main Procedure *)
+
+(** *** f_eval_subprogram_correct *)
+Theorem f_eval_subprogram_correct: forall k s f s',
+    (f_eval_subprogram k s f = Normal s' -> 
+        eval_subprogram s f (Normal s')) /\
+    (f_eval_subprogram k s f = Run_Time_Error -> 
+        eval_subprogram s f Run_Time_Error).
+Proof.
+    intros; 
+    split; intros;
+    destruct f;
+    simpl in H;
+    constructor;
+    unfold f_eval_proc in H;
+    remember (f_eval_decl s nil (procedure_declarative_part p)) as x;
+    symmetry in Heqx.
+  - (* normal state *)
+    destruct x; inversion H; subst.
+    econstructor.
+    + apply f_eval_decl_correct in Heqx.
+       apply Heqx.
+    + apply f_eval_stmt_correct in H.
+       rewrite H1; auto.
+  - (* run time error *)
+    destruct x; inversion H; subst.
+    + econstructor.
+       * apply f_eval_decl_correct in Heqx.
+         apply Heqx.
+       * rewrite H.
+         apply f_eval_stmt_correct in H; auto.
+    + econstructor.
+      apply f_eval_decl_correct2 in Heqx; auto.
+Qed.
+
+(** *** f_eval_subprogram_complete *)
+Theorem f_eval_subprogram_complete: forall s f s',
+    eval_subprogram s f s' ->
+    exists k, f_eval_subprogram k s f = s'.
+Proof.
+    intros s f s' h.
+    unfold f_eval_subprogram.
+    unfold f_eval_proc.
+    inversion h; subst.
+    inversion H; subst.
+  - apply f_eval_decl_complete in H0.
+    rewrite H0. 
+    exists 0; auto.
+  - apply f_eval_decl_complete in H0.
+    rewrite H0.
+    apply f_eval_stmt_complete in H1.
+    auto.
+Qed.
+
+(** * Replaying examples using the correctness of functional semantics *)
+Module ExampleProcedures2.
+(* EXAMPLE 1, v102 is a variable in the scope.
+------------------------
+procedure P2 () is
+  V4 : TYPE5 := 34;
+begin
+  V102 := 56;
+end 
+-----------------------
+*)
+Definition proc1:procedure_body := (mkprocedure_body
+           1 2 nil nil
+             (D_Object_declaration
+                {|
+                  declaration_astnum := 3;
+                  object_name := 4;
+                  object_nominal_subtype :=  5;
+                  initialization_expression := Some (E_Literal 6 (Integer_Literal(34)))
+                |}
+             )
+             (S_Assignment 12 102 (E_Literal 8 (Integer_Literal(56))))).
+
+Definition s1:store := (101,Procedure proc1) :: (102, Value (Int(77))) :: nil.
+
+Definition s2:store := (101,Procedure proc1) :: (102, Value (Int(56)))  :: nil.
+
+Eval vm_compute in f_eval_stmt 200 (s1::nil) (S_ProcCall 13 101 nil).
+
+Lemma essai: eval_stmt (s1::nil) (S_ProcCall 13 101 nil) (Normal (s2::nil)).
+Proof.
+  apply f_eval_stmt_correct1 with (k:=2).
+  compute.
+  reflexivity.
 Qed.
 
 
@@ -445,1491 +2059,13 @@ Definition s3:store := (101,Procedure proc2) :: (102, Value (Int(77))) :: nil.
 Definition s4:store := (101,Procedure proc2) :: (102, Value (Int(142)))  :: nil.
 
 
-Lemma essai2: eval_stmt s3 (S_ProcCall 13 101 nil) (S_Normal s4).
+Lemma essai2: eval_stmt (s3::nil) (S_ProcCall 13 101 nil) (Normal (s4::nil)).
 Proof.
-  eapply eval_S_Proc; try now (simpl; eauto).
-  - simpl.
-    constructor.
-  - simpl List.app.
-    instantiate (1:= ((5, Value (Int 37))::(4, Value (Int 34))::s3)).
-    unfold s3, s4, proc1.
-    simpl.
-    econstructor 4;simpl.
-    + econstructor 2;simpl.
-      * econstructor;eauto.
-      * reflexivity.
-      * constructor.
-        simpl.
-        reflexivity.
-    + econstructor 2;simpl.
-      * econstructor;eauto.
-      * reflexivity.
-      * constructor.
-        simpl.
-        reflexivity.
-  - instantiate (2:=(5, Value (Int 71)) :: (4, Value (Int 34)) :: nil).
-    instantiate (1:=s4).
-    simpl.
-    + { econstructor.
-        - instantiate (1:=(5, Value (Int 71)) :: (4, Value (Int 34)) :: s3).
-          econstructor.
-          + econstructor.
-            * econstructor.
-              simpl.
-              eauto.
-            * constructor.
-              simpl.
-              eauto.
-            * constructor.
-              vm_compute.
-              reflexivity.
-            * econstructor.
-              simpl.
-              eauto.
-          + simpl.
-            reflexivity.
-        - econstructor.
-          + econstructor.
-            * econstructor.
-              simpl.
-              eauto.
-            * econstructor.
-              simpl.
-              eauto.
-            * econstructor.
-              vm_compute.
-              reflexivity.
-            * econstructor.
-            simpl.
-            eauto.
-        + simpl.
-          reflexivity. }
-  - reflexivity.
-  - simpl.
-    constructor 1.
+  apply f_eval_stmt_correct1 with (k:=200).
+  vm_compute.
+  reflexivity.
 Qed.
 
 
-End ExampleProcedures.
+End ExampleProcedures2.
 (* END EXAMPLE *)  
-
-(** ** Functional Semantics of expressions *)
-
-(** for relational semantics of expression and statement, we also 
-    provide its corresponding version of functional semantics, and 
-    prove that they are semantics equivalent;
-    relational semantics encode the formal semantics rules, while
-    functional semantics is useful to familiarize oneself with the 
-    SPARK 2014 semantics, and validate it experimentally by testing, 
-    and it also helps to fix the program if the program exhibits 
-    undefined behavior;
-    
-    Bisimulation between relational and functional semantics are
-    proved for the following pairs of evaluations: 
-    
-    - f_eval_binexpr <-> eval_binexpr;
-    
-    - f_eval_unaryexpr <-> eval_unaryexpr;
-    
-    - f_eval_expr <-> eval_expr;
-
-    - f_eval_stmt <-> eval_stmt;
-*)
-
-(** *** semantic of operators *)
-
-(** interpret the binary operation for each binary operator *)
-Definition f_eval_bin_expr (op: binary_operator) (v1: value) (v2: value): return_val :=
-    match op with
-    | Equal => Val.eq v1 v2
-    | Not_Equal => Val.ne v1 v2
-    | Greater_Than => Val.gt v1 v2
-    | Greater_Than_Or_Equal => Val.ge v1 v2
-    | Less_Than => Val.lt v1 v2
-    | Less_Than_Or_Equal => Val.le v1 v2
-    | And => Val.and v1 v2
-    | Or => Val.or v1 v2
-    | Plus => Val.add v1 v2
-    | Minus => Val.sub v1 v2
-    | Multiply => Val.mul v1 v2
-    | Divide => Val.div v1 v2
-    end.
-
-(** interpret the unary operation *)
-Definition f_eval_unary_expr (op: unary_operator) (v: value): return_val :=
-    match op with
-    | Not => Val.not v
-    end.
-
-(** *** Expression semantics *)
-
-(** in functional semantics for expression, it returns either a
-    normal value or a run time error or go abnormal, the run time 
-    checks (for example, division by zero check) are encoded inside 
-    the semantics; *)
-Function f_eval_expr (s: store) (e: expression): return_val :=
-    match e with
-    | E_Literal _ v => Val_Normal (eval_literal v)
-    | E_Identifier _ x =>
-        match (fetch x s) with
-        | Some (Value v) => Val_Normal v
-        | _ => Val_Abnormal (* None or procedure *)
-        end
-    | E_Binary_Operation _ op e1 e2 =>
-        match f_eval_expr s e1 with
-        | Val_Normal v1 => 
-            match f_eval_expr s e2 with
-            | Val_Normal v2 => 
-                match f_do_check op v1 v2 with
-                | Some true => f_eval_bin_expr op v1 v2
-                | Some false => Val_Run_Time_Error
-                | _ => Val_Abnormal
-                end
-            | Val_Run_Time_Error => Val_Run_Time_Error
-            | Val_Abnormal => Val_Abnormal
-            end
-        | Val_Run_Time_Error => Val_Run_Time_Error
-        | Val_Abnormal => Val_Abnormal
-        end   
-    | E_Unary_Operation _ op e => 
-        match f_eval_expr s e with
-        | Val_Normal v => f_eval_unary_expr op v
-        | Val_Run_Time_Error => Val_Run_Time_Error
-        | Val_Abnormal => Val_Abnormal
-        end
-    end.
-
-(** ** Functional Statement semantics *)
-
-
-(** *** Functional manipulation of the stack for procedure call and
-    retrun *)
-
-(** functional version of Copy_out
-  [copy_out prefx params lexp s'] returns s' updated in the following
-  way: for each param in params that is Out, pick the correponding
-  variable name in lexp and update s' with the value of the param that
-  is stored in prefix. *)
-Function copy_out (prefx:store) (params: list parameter_specification)
-         (lexp:list expression) (s: store) {struct params}:  state :=
-  match params, lexp with
-    | nil , nil => S_Normal s
-    | (prm::params') , (e::lexp') =>
-      match prm.(parameter_mode) with
-         | Out =>
-           match e with
-             | E_Identifier _ x =>
-               match (fetch (prm.(parameter_name)) prefx) with
-                   Some v =>
-                   match update s x v with
-                     | Some s' => copy_out prefx params' lexp' s'
-                     | None => S_Abnormal
-                   end
-                 | None => S_Abnormal
-               end
-             | _ => S_Abnormal
-           end
-         | In => copy_out prefx params' lexp' s
-         | _ => S_Abnormal
-       end
-    | _ , _ => S_Abnormal
-  end.
-
-(** Functional version of Copy_in.
-   [copy_in s lparams lexp] returns the prefix to push on the stack
-   before evaluationg procedure body (i.e. declaration block +
-   statement). "Out" parameters values are copied into there output
-   variables (stored in lexp). *)
-Function copy_in (s:store) lparams lexp: state :=
-  match lparams,lexp with
-  | (prm :: lparams') , (exp:: lexp') =>
-    match prm.(parameter_mode) with
-      | Out => if is_var exp
-               then match copy_in s lparams' lexp' with
-                      | S_Normal res => S_Normal ((prm.(parameter_name), Undefined) :: res)
-                      | res => res
-                    end
-               else S_Abnormal
-      | In =>
-        let v := f_eval_expr s exp in
-        match v with
-          | Val_Normal v' =>
-            match copy_in s lparams' lexp' with
-              | S_Normal res => S_Normal ((prm.(parameter_name), Value v') :: res)
-              | res => res
-            end
-          | Val_Run_Time_Error => S_Run_Time_Error
-          | Val_Abnormal => S_Abnormal
-        end
-      | In_Out => S_Abnormal (* not yet implemented *)
-    end
-  | nil , nil => S_Normal nil
-  | _ , _ => S_Abnormal
-  end.
-
-(** *** functional semantic of declarations *)
-
-Function f_eval_decl (s: store) (c: declaration) {struct c}: state :=
-  match c with
-    | D_Object_declaration d =>
-      match d.(initialization_expression) with
-        | Some e =>
-          match f_eval_expr s e with
-            | Val_Run_Time_Error => S_Run_Time_Error
-            | Val_Normal v =>
-              (S_Normal ((d.(object_name), Value v) :: s))
-            | Val_Abnormal => S_Abnormal
-          end
-        | None => (S_Normal ((d.(object_name), Undefined) :: s))
-      end
-    | D_Sequence dcl1 dcl2 =>
-      match f_eval_decl s dcl1 with
-        | S_Normal s' => f_eval_decl s' dcl2
-        | err => err
-      end
-    | D_Procedure_declaration pbody =>
-      S_Normal((procedure_name pbody,Procedure pbody)::s)
-  end.
-
-(** *** functional semantic of statements *)
-
-(** 
-   in the functional semantics for statement, 'k' denotes the execution 
-   steps, whenever it reaches 0, an untermination state is returned;
-   otherwise, it returns either a normal state, or a run time error 
-   or an abnormal state; run time checks (for example, division by 
-   zero check) are encoded inside the functional semantics;
-*)
-Function f_eval_stmt k (s: store) (c: statement) {struct k}: state := 
-  match k with
-  | 0 => S_Unterminated
-  | S k' => 
-    match c with
-    | S_Assignment ast_num x e =>
-        match f_eval_expr s e with
-        | Val_Normal v => 
-            match update s x (Value v) with
-            | Some s1 => S_Normal s1
-            | None => S_Abnormal
-            end
-        | Val_Run_Time_Error => S_Run_Time_Error
-        | Val_Abnormal => S_Abnormal
-        end
-    | S_Sequence ast_num c1 c2 =>
-        match f_eval_stmt k' s c1 with
-        | S_Normal s1 => f_eval_stmt k' s1 c2
-        | S_Run_Time_Error => S_Run_Time_Error
-        | S_Unterminated => S_Unterminated
-        | S_Abnormal => S_Abnormal
-        end
-    | S_If ast_num b c =>
-        match f_eval_expr s b with
-        | Val_Normal (Bool true) => f_eval_stmt k' s c
-        | Val_Normal (Bool false) => S_Normal s
-        | Val_Run_Time_Error => S_Run_Time_Error
-        | _ => S_Abnormal
-        end
-    | S_While_Loop ast_num b c => 
-        match f_eval_expr s b with
-        | Val_Normal (Bool true) => 
-            match f_eval_stmt k' s c with
-            | S_Normal s1 => f_eval_stmt k' s1 (S_While_Loop ast_num b c)
-            | S_Run_Time_Error => S_Run_Time_Error
-            | S_Unterminated => S_Unterminated
-            | S_Abnormal => S_Abnormal
-            end
-        | Val_Normal (Bool false) => S_Normal s
-        | Val_Run_Time_Error => S_Run_Time_Error
-        | _ => S_Abnormal
-        end
-    | S_ProcCall ast_num pbname lexp =>
-      match fetch pbname s with
-        | Some (Procedure pb) => 
-          match copy_in s (procedure_parameter_profile pb) lexp with
-            | S_Normal prefx => 
-              match f_eval_decl (prefx ++ s) (procedure_declarative_part pb) with
-                | S_Normal s2 =>
-                  match f_eval_stmt k' s2 (procedure_statements pb) with
-                    | S_Normal s3 =>
-                      match split2 (List.length s3 - List.length (prefx ++ s))
-                                   (List.length prefx) s3 with
-                        | Some (slocal,p) =>
-                          match p with
-                            | (prefx',s') =>
-(*                               S_Normal (copy_out prefx (procedure_parameter_profile pb) lexp s3) *)
-                              (copy_out prefx' (procedure_parameter_profile pb) lexp s')
-                          end
-                        | None => S_Abnormal (* erronous stack size *)
-                      end
-                    | S_Run_Time_Error => S_Run_Time_Error
-                    | _ => S_Abnormal
-                  end
-                | S_Run_Time_Error => S_Run_Time_Error
-                | _ => S_Abnormal
-              end
-            | err => err
-          end
-        | _ => (* None or non-procedure *) S_Abnormal
-      end
-    end
-  end.
-
-
-(** basic lemmas *)
-(** expression semantic is deterministic. *)
-Lemma eval_expr_unique: forall s e v1 v2,
-    eval_expr s e (Val_Normal v1) ->
-    eval_expr s e (Val_Normal v2) ->
-    v1 = v2.
-Proof.
-    induction e; 
-    intros v1 v2 h1 h2;
-    inversion h1; subst;
-    inversion h2; subst;
-    auto.
-  - rewrite H1 in H2; 
-    inversion H2; auto.
-  - specialize (IHe1 _ _ H5 H9).
-    specialize (IHe2 _ _ H6 H10).
-    subst.
-    specialize (eval_bin_unique _ _ _ _ _ H8 H12); intros hz1; subst.
-    auto.
-  - specialize (IHe _ _ H3 H5). subst.
-    destruct op, op0.
-    specialize (eval_unary_unique _ _ _ _ H4 H6); intros hz1; subst.
-    auto.
-Qed.
-
-(** 
-    for any expression e evaluated under the state s, if it can be 
-    evaluated to a value v with respect to the relational semantics 
-    eval_expr, then the result value v should be either a normal 
-    value or a run time error;
-*)
-Lemma eval_expr_state : forall s e v,
-        eval_expr s e v -> (* v should be either a normal value or a run time error *)
-            (exists v0, v = Val_Normal v0) \/ v = Val_Run_Time_Error.
-Proof.
-    intros s e v h.
-    induction h;
-    try match goal with
-    | [ |- (exists v, Val_Normal ?v1 = Val_Normal v) \/ _ ]
-      => left; exists v1; reflexivity
-    | [ |- context [ _ \/ ?A = ?A ] ] => right; reflexivity
-    end; auto.
-Qed.
-
-(** 
-    for any statement c starting from the initial state s, if it 
-    terminates in a state s' with respect to the relational semantics 
-    eval_stmt, then the result state s' should be either a normal 
-    state or a run time error. In relational semantics eval_stmt, 
-    all statements that can go abnormal are excluded;
-*)
-Lemma eval_stmt_state : forall s c s',
-        eval_stmt s c s' -> (* s' is either a normal state or a run time error *)
-            (exists v, s' = S_Normal v) \/ s' = S_Run_Time_Error.
-Proof.
-    intros s c s' h.
-    induction h;
-    try match goal with
-    | [ |- (exists v, S_Normal ?v1 = S_Normal v) \/ _ ] => left; exists v1; reflexivity
-    | [ |- context [ _ \/ ?A = ?A ] ] => right; reflexivity
-    end; auto.
-Qed.
-
-(** * Bisimulation Between Relational And Functional Semantics *)
-
-(** bisimulation proof between f_eval_binexpr and eval_binexpr:
-    - f_eval_bin_expr_correct
-    - f_eval_bin_expr_complete
-*)
-Lemma f_eval_bin_expr_correct: forall op v1 v2 v,
-    f_eval_bin_expr op v1 v2 = Val_Normal v ->
-    eval_bin_expr op v1 v2 v.
-Proof.
-    intros op v1 v2 v h1.
-    destruct op;
-    match goal with 
-    |[|- eval_bin_expr Divide _ _ _] => idtac
-    |[|- eval_bin_expr ?op _ _ _] =>
-        destruct v1, v2;
-        simpl in h1; inversion h1; subst;
-        constructor; auto
-    end.
-    destruct v1, v2; simpl in h1; inversion h1.
-    constructor.
-    remember (Zeq_bool n0 0) as x.
-    reflexivity.
-Qed.
-
-Lemma f_eval_bin_expr_complete: forall op v1 v2 v,
-    eval_bin_expr op v1 v2 v ->
-    f_eval_bin_expr op v1 v2 = Val_Normal v.
-Proof.
-    intros op v1 v2 v h1.
-    induction h1;
-    rewrite <- H;
-    simpl; auto.
-Qed.
-
-(** bisimulation proof between f_eval_unaryexpr and eval_unaryexpr: 
-    - f_eval_unary_expr_correct
-    - f_eval_unary_expr_complete
-*)
-Lemma f_eval_unary_expr_correct: forall op v v',
-    f_eval_unary_expr op v = Val_Normal v' ->
-    eval_unary_expr op v v'.
-Proof.
-    intros.
-    destruct op; simpl in H.
-    destruct v; inversion H; subst.
-    constructor; auto.
-Qed.
-
-Lemma f_eval_unary_expr_complete: forall op v v',
-    eval_unary_expr op v v' ->
-    f_eval_unary_expr op v = Val_Normal v'.
-Proof.
-    intros op v v' h1;
-    induction h1;
-    rewrite <- H;
-    simpl; auto.
-Qed.
-
-(** ** Bisimulation between f_eval_expr and eval_expr for expression Semantics *)
-(** a help lemma to prove the theorem: f_eval_expr_correct *)
-Lemma f_eval_expr_correct1 : forall s e v,
-                        f_eval_expr s e = Val_Normal v ->
-                            eval_expr s e (Val_Normal v).
-Proof.
-    intros s e.
-    functional induction (f_eval_expr s e);
-    intros v0 h1;
-    try inversion h1; subst.
-  - constructor;
-    reflexivity.
-  - constructor;
-    assumption.
-  - specialize (IHr _ e3).
-    specialize (IHr0 _ e4).
-    rewrite H0.
-    econstructor.
-    exact IHr. exact IHr0.
-    + apply f_do_check_correct.
-      auto.
-    + apply f_eval_bin_expr_correct; 
-      auto.
-  - specialize (IHr _ e2).
-    rewrite h1.
-    econstructor. 
-    exact IHr.
-    destruct op. 
-    simpl in h1. 
-    destruct v; inversion h1; subst.
-    constructor; auto.
-Qed.
-
-(** another help lemma to prove the theorem: f_eval_expr_correct *)
-Lemma f_eval_expr_correct2 : forall s e,
-                        f_eval_expr s e = Val_Run_Time_Error ->
-                            eval_expr s e Val_Run_Time_Error.
-Proof.
-    intros s e.
-    functional induction (f_eval_expr s e);
-    intros h; try inversion h.
-  - destruct op, v1, v2;
-    simpl in h; inversion h.
-  - specialize (f_eval_expr_correct1 _ _ _ e3); intros hz1.
-    specialize (f_eval_expr_correct1 _ _ _ e4); intros hz2.
-    eapply eval_E_Binary_Operation3.
-    apply hz1. apply hz2.
-    apply f_do_check_correct; auto.
-  - specialize (f_eval_expr_correct1 _ _ _ e3); intros hz1.
-    specialize (IHr0 e4).
-    eapply eval_E_Binary_Operation2; auto.
-    exact hz1.
-  - specialize (IHr e3).
-    constructor; assumption.
-  - destruct op;
-    destruct v; inversion h. 
-  - specialize (IHr e2).
-    constructor; assumption.
-Qed.
-
-(** *** f_eval_expr_correct *)
-(** 
-    for an expression e evaluated under the state s with respect to
-    the functional semantics f_eval_expr, whenever it returns a 
-    normal value v or terminates in a run time error, 
-    the relation between s, e and evaluation result should also be 
-    satisfied with respect to the relational semantics 'eval_expr';
-*)
-Theorem f_eval_expr_correct : forall s e v,
-                        (f_eval_expr s e = Val_Normal v ->
-                            eval_expr s e (Val_Normal v)) /\
-                        (f_eval_expr s e = Val_Run_Time_Error ->
-                            eval_expr s e Val_Run_Time_Error).
-Proof.
-    split.
-  - apply f_eval_expr_correct1.
-  - apply f_eval_expr_correct2.
-Qed.
-
-
-(** *** f_eval_expr_complete *)
-(** 
-   for any expression e, if it can be evaluated to a value v under
-   state s with respect to the relational semantics 'eval_expr', 
-   then when we evalute e under the same state s in functional
-   semantics 'f_eval_expr', it should return the same result v;
-*)
-Theorem f_eval_expr_complete : forall e s v,  
-                        eval_expr e s v -> 
-                            (f_eval_expr e s) = v.
-Proof.
-    intros e s v h.
-    induction h; simpl; intros;
-    repeat match goal with
-    | h: fetch _ _ = _  |- _ => progress rewrite h
-    | h: f_eval_expr _ _ = _ |- _ => progress rewrite h
-    end;auto.
-  - rewrite H; reflexivity.
-  - specialize (f_do_check_complete _ _ _ _ H); intros hz1.
-    rewrite hz1.
-    reflexivity.
-  - destruct v1; destruct v2;
-    destruct op;
-    inversion H0; subst; simpl; auto.
-    + (* overflow check for Plus *)
-      inversion H; subst.
-      rewrite H3; auto.
-      unfold not in H2; intuition.
-    + (* overflow check for Minus *)
-      inversion H; subst.
-      rewrite H3; auto.
-      unfold not in H2; intuition.
-    + (* overflow check for Multiply *)
-      inversion H; subst.
-      rewrite H3; auto.
-      unfold not in H2; intuition.
-    + (* both division by zero check and overflow check *)
-      inversion H; subst.
-      rewrite H3; auto.
-      rm_false_hyp.
-  - destruct op.
-    inversion H; subst.
-    auto.
-Qed.
-
-Ltac apply_inv :=
-  match goal with
-    | H:S_Unterminated = S_Normal _ |- _ => inversion H
-    | H:S_Unterminated = S_Run_Time_Error |- _ => inversion H
-    | H:S_Unterminated = S_Abnormal |- _ => inversion H
-    | H:S_Abnormal = S_Normal _ |- _ => inversion H
-    | H:S_Abnormal = S_Run_Time_Error |- _ => inversion H
-    | H:S_Abnormal = S_Unterminated |- _ => inversion H
-    | H:S_Run_Time_Error = S_Normal _ |- _ => inversion H
-    | H:S_Run_Time_Error = S_Abnormal |- _ => inversion H
-    | H:S_Run_Time_Error = S_Unterminated |- _ => inversion H
-    | H:S_Normal _ = S_Unterminated |- _ => inversion H
-    | H:S_Normal _ = S_Run_Time_Error |- _ => inversion H
-    | H:S_Normal _ = S_Abnormal |- _ => inversion H
-    | H:S_Normal _ = S_Normal _ |- _ => inversion H;clear H;subst 
-    | H:update _ _ (Value _) = _ |- _ => rewrite H
-    | H:f_eval_stmt _ _ _ = _ |- _ => rewrite H
-    | H:f_eval_expr _ _ = _ |- _ => rewrite H
-    | H:f_eval_decl _ _ = _ |- _ => rewrite H
-    | H:copy_out _ _ _ _ = _ |- _ => rewrite H
-    | H:copy_in _ _ _ = _ |- _ => rewrite H
-    | H:fetch _ _ = _ |- _ => rewrite H
-    | H:split2 _ _ _ = _ |- _ => rewrite H
-  end;subst;simpl;auto.
-
-Ltac invle := match goal with
-    | H: (S _ <= _)%nat |- _ => (inversion H; clear H; subst; simpl)
-  end.
-
-(** a help lemma to prove the theorem: 'f_eval_stmt_complete',
-    it means that: for any statement c, starting from initial state s, 
-    if it terminates in a normal state s' within k execution steps, 
-    then for any k' greater and equal than k, it should also terminate 
-    in the same state s';
-*)
-Lemma f_eval_stmt_fixpoint: forall k s c s', 
-        f_eval_stmt k s c = S_Normal s' ->
-        forall k':nat, (k <= k')%nat -> 
-            f_eval_stmt k' s c = S_Normal s'.
-Proof.
-    intros k s c.
-    functional induction (f_eval_stmt k s c); simpl; intros; subst; simpl; auto;
-    repeat progress apply_inv.
-  - invle; repeat apply_inv.
-  - invle.
-    + repeat apply_inv.
-    + rewrite (IHs0 _ e1);auto with arith.
-  - invle; repeat apply_inv. rewrite (IHs0 _ H);auto with arith.
-  - invle; repeat apply_inv.
-  - invle; repeat apply_inv. rewrite (IHs0 _ e2); auto with arith.
-  - invle; repeat apply_inv.
-  - invle; repeat apply_inv.
-    + rewrite (IHs0 _ e4).
-      repeat apply_inv.
-      auto with arith.
-  - invle.
-    + rewrite H in *.
-      contradiction.
-    + rewrite H in *.
-      contradiction.
-Qed.
-
-(** another help lemma to prove the theorem: 'f_eval_stmt_complete' *)
-Lemma f_eval_stmt_fixpoint_E: forall k s p, 
-        f_eval_stmt k s p = S_Run_Time_Error ->
-        forall k':nat, (k <= k')%nat -> 
-            f_eval_stmt k' s p = S_Run_Time_Error.
-Proof.
-    intros k s p.
-    functional induction (f_eval_stmt k s p); simpl; intros; subst; simpl; auto;
-    repeat progress apply_inv. 
-  - invle;
-    apply_inv.
-  - invle;
-    repeat apply_inv.
-    rewrite (f_eval_stmt_fixpoint _ _ _ _ e1); auto with arith.
-  - invle;
-    repeat apply_inv.
-    specialize (IHs0 e1). 
-    rewrite IHs0; auto with arith. 
-  - invle; 
-    repeat apply_inv.
-    rewrite IHs0; auto with arith.
-  - invle;
-    repeat apply_inv.
-  - invle; 
-    repeat apply_inv. 
-    rewrite (f_eval_stmt_fixpoint _ _ _ _ e2); auto with arith.
-  - invle; 
-    repeat apply_inv.
-    rewrite (IHs0 e2); auto with arith.    
-  - invle; 
-    repeat apply_inv.   
-  - invle; repeat apply_inv.
-    rewrite (f_eval_stmt_fixpoint _ _ _ _ e4); auto with arith.
-    rewrite e5.
-    assumption.
-  - invle; repeat apply_inv.
-    rewrite  (IHs0 e4 m);auto with arith.
-  - clear H.
-    invle; repeat apply_inv.
-  - invle; repeat apply_inv.
-Qed.
-
-
-Ltac destrIH :=
-  repeat progress (match goal with
-                     | h: ex _ |- _  =>
-                       let k := fresh "k" in
-                       let hk1 := fresh "hk" in
-                       destruct (h) as [k hk1];try assumption
-                   end).
-
-Ltac kgreater :=
-  repeat
-    match goal with
-      | h:f_eval_stmt ?k ?s ?p = S_Normal ?s' |- context [f_eval_stmt (?k + _) ?s ?p] =>
-        rewrite (@f_eval_stmt_fixpoint _ _ _ _ h);auto with arith
-      | h:f_eval_stmt ?k ?s ?p = S_Normal ?s' |- context [f_eval_stmt (_ + ?k) ?s ?p] =>
-        rewrite (@f_eval_stmt_fixpoint _ _ _ _ h);auto with arith
-      | h:f_eval_stmt ?k ?s ?p = S_Run_Time_Error |- context [f_eval_stmt (?k + _) ?s ?p] =>
-        rewrite (@f_eval_stmt_fixpoint_E _ _ _ h);auto with arith
-      | h:f_eval_stmt ?k ?s ?p = S_Run_Time_Error |- context [f_eval_stmt (_ + ?k) ?s ?p] =>
-        rewrite (@f_eval_stmt_fixpoint_E _ _ _ h);auto with arith
-         end.
-
-
-Ltac rm_f_eval_expr :=
-  match goal with 
-    | [ h: f_eval_expr ?s ?b = Val_Run_Time_Error |- _ ] => 
-      specialize (f_eval_expr_correct2 _ _ h); intros hz1
-    | [ h: f_eval_expr ?s ?b = Val_Normal ?v |- _ ] => 
-      specialize (f_eval_expr_correct1 _ _ _ h); intros hz1   
-  (*
-    | [ h: f_eval_stmt ?k ?s ?c = S_Run_Time_Error |- _ ] => specialize (f_eval_stmt_correct1 _ _ _ _ h); intros hz1
-    | [ h: f_eval_stmt ?k ?s ?c = S_Normal ?s1 |- _ ] => specialize (f_eval_stmt_correct1 _ _ _ _ h); intros hz1
-   *)
-  end; auto.
-
-Lemma copy_in_correct:
-  forall s prm lexp prefx,
-    copy_in s prm lexp = (S_Normal prefx) <->  Copy_in s prm lexp (S_Normal prefx).
-Proof.
-  intros s prm lexp.
-  functional induction copy_in s prm lexp;intros;split;simpl in *;intro heq
-  ; try (inversion heq;subst;clear heq)
-  ; try (now repeat progress
-           match goal with
-             | HH: ?x = In , HH': ?x = Out |- _ =>
-               rewrite HH in HH'; inversion HH'
-             | HH: ?x = In , HH': ?x = In_Out |- _ =>
-               rewrite HH in HH' ; inversion HH'
-             | HH: ?x = In_Out , HH': ?x = Out |- _ =>
-               rewrite HH in HH'; inversion HH'
-             | H: copy_in _ _ _ = S_Normal ?res , H': forall _, _ <-> _ |- _ =>
-               rewrite <- H' in *
-             | H: Copy_in _ _ _ _ , H': forall _, _ <-> _ |- _ =>
-               rewrite <- H' in *
-             | HH: copy_in ?x ?y ?z = _ , HH': context C [copy_in ?x ?y ?z = _] |- _ =>
-               (rewrite HH in HH'; inversion HH' ; subst)
-             | HH: copy_in ?x ?y ?z = _ , H': forall _, _ <-> _  |- _  =>
-               rewrite HH in *; contradiction
-             | H1: f_eval_expr ?s ?exp = Val_Abnormal,
-                   H2: eval_expr ?s ?exp (Val_Normal _) |- _ =>
-               apply f_eval_expr_complete in H2
-             ; rewrite H2 in H1
-             ; inversion H1
-             | H1: f_eval_expr ?s ?exp = (Val_Normal _),
-                   H2: eval_expr ?s ?exp (Val_Normal _) |- _ =>
-               apply f_eval_expr_complete in H2;
-             rewrite H2 in H1;
-             inversion H1
-             | H1: f_eval_expr ?s ?exp = Val_Run_Time_Error,
-                   H2: eval_expr ?s ?exp (Val_Normal _) |- _ =>
-               apply f_eval_expr_complete in H2;
-             rewrite H2 in H1;
-             inversion H1
-           end ; auto);
-  try match goal with
-    | H: is_var ?e = true |- _ =>
-      rewrite is_var_Is_var in H
-      ; destruct e;simpl in H; try contradiction;subst
-  end.
-
-  - econstructor 2.
-    + apply IHs0;auto.
-    + assumption.
-
-  - apply Copy_in_cons_in.
-    + apply IHs0.
-      assumption.
-    + assumption.
-    + apply f_eval_expr_correct1.
-      assumption.
-  - constructor 1.
-Qed.
-
-Lemma copy_in_correct2:
-  forall s prm lexp,
-    copy_in s prm lexp = S_Run_Time_Error <->  Copy_in s prm lexp S_Run_Time_Error.
-Proof.
-  intros s prm lexp.
-  functional induction copy_in s prm lexp;intros;split;simpl in *;intro heq
-  ; try (inversion heq;subst;clear heq)
-  ; try (now repeat progress
-           match goal with
-             | HH: ?x = In , HH': ?x = Out |- _ =>
-               rewrite HH in HH'; inversion HH'
-             | HH: ?x = In , HH': ?x = In_Out |- _ =>
-               rewrite HH in HH' ; inversion HH'
-             | HH: ?x = In_Out , HH': ?x = Out |- _ =>
-               rewrite HH in HH'; inversion HH'
-             | H: copy_in _ _ _ = S_Normal ?res , H': forall _, _ <-> _ |- _ =>
-               rewrite <- H' in *
-             | H: Copy_in _ _ _ _ , H': forall _, _ <-> _ |- _ =>
-               rewrite <- H' in *
-             | HH: copy_in ?x ?y ?z = _ , HH': context C [copy_in ?x ?y ?z = _] |- _ =>
-               (rewrite HH in HH'; inversion HH' ; subst)
-             | HH: copy_in ?x ?y ?z = _ , H': forall _, _ <-> _  |- _  =>
-               rewrite HH in *; contradiction
-             | H1: f_eval_expr ?s ?exp = Val_Abnormal,
-                   H2: eval_expr ?s ?exp (Val_Normal _) |- _ =>
-               apply f_eval_expr_complete in H2
-             ; rewrite H2 in H1
-             ; inversion H1
-             | H1: f_eval_expr ?s ?exp = (Val_Normal _),
-                   H2: eval_expr ?s ?exp (Val_Normal _) |- _ =>
-               apply f_eval_expr_complete in H2;
-             rewrite H2 in H1;
-             inversion H1
-             | H1: f_eval_expr ?s ?exp = Val_Run_Time_Error,
-                   H2: eval_expr ?s ?exp (Val_Normal _) |- _ =>
-               apply f_eval_expr_complete in H2;
-             rewrite H2 in H1;
-             inversion H1
-           end ; auto);
-  try match goal with
-    | H: is_var ?e = true |- _ =>
-      rewrite is_var_Is_var in H
-      ; destruct e;simpl in H; try contradiction;subst
-  end.
-  - rewrite <- IHs0 in H3.
-    rewrite e3 in H3.
-    discriminate.
-  - rewrite H0.
-    econstructor;auto.
-    rewrite <- IHs0.
-    assumption.
-  - apply IHs0.
-    assumption.
-  - rewrite (f_eval_expr_complete s exp _ H5) in e2.
-    discriminate.
-  - rewrite <- IHs0 in H4.
-    rewrite e3 in H4.
-    discriminate.
-
-  - rewrite H0.
-    apply Copy_in_cons_in_rte2 with (v:=v');auto.
-    + rewrite <- IHs0.
-      assumption.
-    + apply (f_eval_expr_correct1).
-      assumption.
-
-  - rewrite (f_eval_expr_complete s exp _ H5) in e2.
-    discriminate.
-  - apply IHs0.
-    assumption.
-  - apply Copy_in_cons_in_rte1;auto.
-    apply f_eval_expr_correct2.
-    assumption.
-  - rewrite (f_eval_expr_complete _ _ _ H5) in e2.
-    discriminate.
-Qed.
-
-
-Lemma Copy_out_length :
-  forall prefx prm lexp s s',
-    Copy_out prefx prm lexp s s'
-    -> List.length s = List.length s'.
-Proof.
-  intros prefx prm lexp s s' H.
-  induction H;auto.
-  transitivity (List.length σ');auto.
-  apply update_length in H2.
-  assumption.
-Qed.
-
-Lemma copy_out_no_rte:
-  forall prefx lprm lexp s,
-    ~ copy_out prefx lprm lexp s = S_Run_Time_Error.
-Proof.
-  intros prefx lprm lexp s.
-  functional induction copy_out prefx lprm lexp s;try assumption;try discriminate.
-Qed.
-
-
-Lemma copy_out_correct:
-  forall prefx s (prm:list parameter_specification) lexp x,
-    copy_out prefx prm lexp s = S_Normal x <-> Copy_out prefx prm lexp s x.
-Proof.
-  intros prefx s prm lexp.
-  Opaque fetch.
-  functional induction copy_out prefx prm lexp s;intros;split;simpl in *;intro heq
-  ; try (now (inversion heq;subst;clear heq);auto;try now (econstructor;eauto)).
-  - apply Copy_out_cons_out with (σ':=s') (v:=v)(id:=parameter_name prm);auto.
-    apply IHs0.
-    assumption.
-  - inversion heq;subst.
-    + rewrite e4 in *.
-      inversion H9;clear H9.
-      subst.
-      apply IHs0.
-      rewrite H10 in *.
-      inversion e5. clear e5. subst.
-      assumption.
-    + rewrite e2 in *.
-      discriminate.
-  - inversion heq;clear heq;subst.
-    + rewrite e4 in *.
-      inversion H9;clear H9.
-      subst.
-      rewrite H10 in *.
-      inversion e5.
-    + rewrite e2 in *.
-      discriminate.
-  - inversion heq;clear heq;subst.
-    + rewrite e4 in *.
-      inversion H9.
-    + rewrite e2 in *.
-      discriminate.
-  - inversion heq;subst;try contradiction.
-    rewrite e2 in *.
-    discriminate.
-  - constructor 3;auto.
-    apply IHs0.
-    assumption.
-  - inversion heq;subst;try contradiction.
-    + rewrite e2 in *.
-      discriminate.
-    + apply IHs0.
-      assumption.
-  - inversion heq;subst;try contradiction.
-    + rewrite H3 in *;contradiction.
-    + rewrite H6 in *;contradiction.
-Qed.
-
-
-
-
-
-Lemma eval_decl_store_length:
-  forall s s' decl,
-    eval_decl s decl s'
-    -> forall st, s' = S_Normal st
-                  -> exists prfx, st = prfx ++ s.
-Proof.
-  intros s s' decl h.
-  induction h;intros st heq;inversion heq;clear heq;subst.
-  - exists ((object_name d, Value v)::nil).
-    simpl.
-    reflexivity.
-  - exists ((object_name d, Undefined)::nil);simpl.
-    reflexivity.
-  - destruct (IHh2 st).
-    { reflexivity. }
-    destruct (IHh1 s').
-    { reflexivity. }
-    subst.
-    exists (x ++ x0).
-    apply app_assoc.
-  - exists ((procedure_name pbody, Procedure pbody)::nil);simpl.
-    reflexivity.
-Qed.
-
-
-Lemma eval_stmt_store_length:
-  forall s s' stm,    
-    eval_stmt s stm s'
-    -> forall st, s' = S_Normal st
-                  -> List.length s = List.length st.
-Proof.
-  intros s s' stm H.
-  induction H;intros st heq;inversion heq;clear heq; subst;auto.
-  - apply update_length in H0.
-    assumption.
-  - transitivity (List.length s1).
-    + apply IHeval_stmt1;auto.
-    + apply IHeval_stmt2;auto.
-  - transitivity (List.length s1).
-    + apply IHeval_stmt1;auto.
-    + apply IHeval_stmt2;auto.
-  - apply eval_decl_store_length with (st:=s2) in H2.
-    + transitivity (List.length s').
-      * symmetry;assumption.
-      * apply Copy_out_length in H7.
-        assumption.
-    + reflexivity.
-Qed.
-
-Lemma f_eval_decl_correct :
-  forall s d s',
-    f_eval_decl s d = S_Normal s' ->
-    eval_decl s d (S_Normal s').
-Proof.
-  intros s d.
-  functional induction f_eval_decl s d;simpl;intros;try discriminate;
-  try match goal with
-        | H: S_Normal _ = S_Normal _ |- _ =>
-          inversion H;subst;clear H
-      end;try now( (econstructor;eauto);try apply f_eval_expr_correct1;auto).
-
-  - destruct (f_eval_decl s dcl1);try contradiction; discriminate.
-Qed.
-
-Lemma f_eval_decl_correct2 :
-  forall s d,
-    f_eval_decl s d = S_Run_Time_Error ->
-    eval_decl s d S_Run_Time_Error.
-Proof.
-  intros s d.
-  functional induction f_eval_decl s d;simpl;intros;try discriminate;
-  try match goal with
-        | H: S_Normal _ = S_Run_Time_Error |- _ =>
-          inversion H;subst;clear H
-      end;try now( (econstructor;eauto);try apply f_eval_expr_correct2;auto).
-  
-  eapply eval_decl_Seq_err2 with s';auto.
-  apply f_eval_decl_correct.
-  assumption.
-Qed.
-
-Ltac invclear H := inversion H; clear H; subst.
-
-Ltac use_determinism :=
-  match goal with
-    | H : ?X = ?X |- _ => clear H
-    | H: None = ?y, H': ?y = Some ?z |- _ => rewrite H' in H; invclear H
-    | H: Some ?z = ?y, H': ?y = None |- _ => rewrite H' in H; invclear H
-    | H: Some ?x = ?y, H': ?y = Some ?z |- _ => rewrite H' in H; inversion H;clear H;subst
-    | H : eval_expr ?s ?e ?X,
-          H': f_eval_expr ?s ?e = ?Y |- _
-      => rewrite (f_eval_expr_complete s e X H) in H'
-    | H:  eval_expr ?s ?e ?X,
-          H': eval_expr ?s ?e ?Y |- _
-      => apply (f_eval_expr_complete s e X) in H
-         ;apply (f_eval_expr_complete s e) in H'
-    | H : f_eval_expr ?s ?e = ?X,
-          H': f_eval_expr ?s ?e = ?Y |- _
-      => rewrite H in H'; invclear H'
-    | H : (Val_Normal ?v) = (Val_Normal ?v') |- _
-      => invclear H
-  end.
-
-Ltac crush := repeat progress use_determinism;try reflexivity;try discriminate.
-
-Lemma f_eval_decl_complete :
-  forall d s s',
-    eval_decl s d s' ->
-    f_eval_decl s d = s'.
-Proof.
-  intros d s.
-  functional induction f_eval_decl s d;simpl;intros;try discriminate;crush;
-  try now (invclear H;crush).
-  - invclear H.
-    + apply IHs0 in H3.
-      rewrite e0 in H3.
-      inversion H3.
-      subst.
-      apply IHs1 in H5.
-      assumption.
-    + apply IHs0 in H4.
-      rewrite e0 in H4.
-      inversion H4.
-    + apply IHs0 in H3.
-      rewrite e0 in H3.
-      inversion H3.
-      subst.
-      apply IHs1 in H5.
-      assumption.
-  - invclear H.
-    + apply IHs0 in H3.
-      rewrite H3 in y.
-      contradiction.
-    + apply IHs0 in H4.
-      assumption.
-    + apply IHs0 in H3.
-      rewrite H3 in y.
-      contradiction.
-Qed.
-
-
-(** ** Bisimulation between f_eval_stmt and eval_stmt for statement semantics *)
-
-
-
-(** a help lemma to prove the theorem: 'f_eval_stmt_complete' *)
-Lemma f_eval_stmt_correct1 : forall k s p s',
-        f_eval_stmt k s p = S_Normal s' ->
-          eval_stmt s p (S_Normal s').
-Proof.
-    intros k s p.
-    functional induction (f_eval_stmt k s p);
-    intros; try inversion H; subst.
-  - (* S_Assignment *)
-    econstructor.
-    rm_f_eval_expr.
-    apply hz1.
-    assumption.
-  - (* S_Sequence *)
-    specialize (IHs0 _ e1).
-    specialize (IHs1 _ H).
-    econstructor.
-    apply IHs0.
-    apply_inv.
-  - (* S_If_True *)
-    specialize (IHs0 _ H).
-    econstructor.
-    rm_f_eval_expr. 
-    apply_inv.
-  - (* S_If_False *)
-    eapply eval_S_If_False.
-    rm_f_eval_expr.
-  - (* S_While_Loop_True *)
-    specialize (IHs0 _ e2).
-    specialize (IHs1 _ H).
-    econstructor.
-    rm_f_eval_expr.
-    apply IHs0. 
-    apply_inv.
-  - (* S_While_Loop_False *)
-    eapply eval_S_While_Loop_False.
-    rm_f_eval_expr.
-  - (* S_ProcCall *)
-    clear H.
-    apply split2_correct in e5.
-    decompose [and] e5 ; clear e5.
-    rewrite H1.
-    eapply eval_S_Proc with (s':=s') (prefix':=prefx')(prefix:=prefx)(slocal:=slocal);eauto.
-    + eapply copy_in_correct.
-      apply e2.
-    + apply f_eval_decl_correct.
-      eassumption.
-    + apply f_eval_decl_correct in e3.
-      destruct (eval_decl_store_length (prefx ++ s) (S_Normal s2) (procedure_declarative_part pb) e3 s2).
-      { reflexivity. }
-      specialize (IHs0 s3 e4).
-      generalize (eval_stmt_store_length _ _ _ IHs0 s3 refl_equal);intros .
-      subst.
-
-      repeat setoid_rewrite app_length in H2.
-      repeat setoid_rewrite app_length in H4.
-      omega.
-    + rewrite <- copy_out_correct.
-      assumption.
-  - rewrite H in y.
-    contradiction.            
-Qed.
-
-
-Ltac rm_f_eval_stmt :=
-    match goal with 
-    | [ h: f_eval_stmt ?k ?s ?c = S_Normal ?s1 |- _ ] => 
-        specialize (f_eval_stmt_correct1 _ _ _ _ h); intros hz1
-    end; auto.
-
-(** a help lemma to prove the theorem: 'f_eval_stmt_complete' *)
-Lemma f_eval_stmt_correct2 : forall k s p,
-        f_eval_stmt k s p = S_Run_Time_Error ->
-          eval_stmt s p S_Run_Time_Error.
-Proof.
-    intros k s p.
-    functional induction (f_eval_stmt k s p);
-      intros H ; try inversion H;  subst.
-  - (* S_Assignment *)
-    econstructor.
-    rm_f_eval_expr.
-  - (* S_Sequence*)
-    specialize (IHs1 H).
-    econstructor.
-    rm_f_eval_stmt.
-    apply hz1.
-    apply_inv.
-  - specialize (IHs0 e1).
-    econstructor.
-    assumption.    
-  - (* C_If *)
-    specialize (IHs0 H).
-    econstructor.
-    rm_f_eval_expr.
-    apply_inv.
-  - econstructor.
-    specialize (f_eval_expr_correct2 _ _ e1); intros hz1. 
-    assumption.
-  - (* S_While_Loop *)
-    specialize (IHs1 H).
-    econstructor.
-    rm_f_eval_expr.
-    rm_f_eval_stmt.
-    apply hz1.
-    apply_inv.
-  - constructor 9.
-    rm_f_eval_expr.
-    specialize (IHs0 e2); assumption.    
-  - econstructor.
-    rm_f_eval_expr.
-
-
-
-  - elim (copy_out_no_rte _ _ _ _ H1).
-  - eapply eval_S_Proc_rtebody with (prefix:=prefx);eauto.
-    + apply copy_in_correct.
-      assumption.
-    + eapply f_eval_decl_correct.
-      assumption.
-  - eapply eval_S_Proc_rtedecl with (prefix:=prefx);eauto.
-    + apply copy_in_correct.
-      assumption.
-    + eapply f_eval_decl_correct2.
-      assumption.
-  - rewrite H.
-    eapply eval_S_Proc_rteargs with pb;auto.
-    apply copy_in_correct2.
-    assumption.
-Qed.
-    
-    
-
-Ltac rm_f_eval :=
-    match goal with 
-    | [ h: f_eval_expr ?s ?b = Val_Run_Time_Error |- _ ] => specialize (f_eval_expr_correct2 _ _ h); intros hz1
-    | [ h: f_eval_expr ?s ?b = Val_Normal ?v |- _ ] => specialize (f_eval_expr_correct1 _ _ _ h); intros hz1   
-    | [ h: f_eval_stmt ?k ?s ?c = S_Run_Time_Error |- _ ] => specialize (f_eval_stmt_correct2 _ _ _ h); intros hz1
-    | [ h: f_eval_stmt ?k ?s ?c = S_Normal ?s1 |- _ ] => specialize (f_eval_stmt_correct1 _ _ _ _ h); intros hz1
-    end; auto.
-
-(** *** f_eval_stmt_correct *)
-(** 
-   for any statement c starting from initial state s, if it returns 
-   a normal state s' or terminates in a run time error within k steps
-   with respect to the functional semantics 'f_eval_stmt', then the 
-   relation between s, c and the resulting state should also be 
-   satisfied with respect to the relational semantics 'eval_stmt';
-*)
-Theorem f_eval_stmt_correct : forall k s c s',
-        (f_eval_stmt k s c = S_Normal s' ->
-          eval_stmt s c (S_Normal s')) /\ 
-        (f_eval_stmt k s c = S_Run_Time_Error ->
-          eval_stmt s c S_Run_Time_Error).
-Proof.
-    intros.
-    split; intros;
-    rm_f_eval.
-Qed.
-
-(** *** f_eval_stmt_complete *)
-(** 
-   the reverse direction is also satisfied: for any statement c, 
-   whenever it's executed starting from initial state s and return 
-   a new state s' with regard to the relational semantics 'eval_stmt', 
-   then there should exist a constant k that statement c starting from 
-   s will terminate in state s' within k steps with respect to the 
-   functional semantics 'f_eval_stmt';
-*)
-
-Ltac apply_rewrite := 
-    match goal with
-    | h: eval_expr ?s ?e ?s' |- _ => 
-        rewrite (f_eval_expr_complete _ _ _ h)
-    | h: update _ _ _ = _ |- _ => rewrite h
-    | h: f_eval_stmt _ _ _ = _ |- _ => rewrite h
-    | h: f_eval_expr _ _ = _ |- _ => rewrite h
-    | h: fetch _ _ = _ |- _ => rewrite h
-    | h: copy_in _ _ _ = _ |- _ => rewrite h
-    | h: Copy_in _ _ _ S_Run_Time_Error |- _ => rewrite <- copy_in_correct2 in h;rewrite h
-    | h: Copy_in _ _ _ (S_Normal _) |- _ => rewrite <- copy_in_correct in h;rewrite h
-    end; auto.
-
-Theorem f_eval_stmt_complete : forall s c s',
-        eval_stmt s c s' -> (* s' is either a normal state or a run time error *)
-            exists k, f_eval_stmt k s c = s'.
-Proof. 
-  intros s c s' H;
-  induction H;
-  try match goal with
-  [ h: eval_expr ?s ?e Val_Run_Time_Error |- exists k, _ = S_Run_Time_Error] => 
-          exists 1%nat; simpl;
-          rewrite (f_eval_expr_complete _ _ _ h);
-          reflexivity
-  end.
-  (* 1. S_Assignment *)
-  - exists 1%nat; simpl.
-    repeat apply_rewrite.
-  (* 2. S_Sequence *)
-  - destrIH.
-    exists (S k); simpl.
-    apply_rewrite.
-  - destrIH.
-    exists (S (k0+k)); simpl.
-    kgreater.
-    specialize (eval_stmt_state _ _ _ H0); intros hz1.
-    destruct hz1 as [hz2 | hz2]; try rm_exists; subst;
-    kgreater.
-  (* 3. S_If *)
-  - destrIH.
-    exists (S k); simpl.
-    apply_rewrite.
-  - exists 1%nat; simpl.
-    apply_rewrite.
-  (* 4. S_While_Loop *)
-  - destrIH.
-    exists (S k); simpl.
-    repeat apply_rewrite.
-  - destrIH.
-    exists (S (k0+k)); simpl.
-    apply_rewrite.
-    kgreater.
-    specialize (eval_stmt_state _ _ _ H1); intros hz1.
-    destruct hz1 as [hz2 | hz2]; try rm_exists; subst;
-    kgreater.
-  - exists 1%nat; simpl.
-    apply_rewrite.
-  - exists 1%nat; simpl.
-    repeat progress apply_rewrite.
-  - exists 1%nat; simpl.
-    subst.
-    repeat apply_rewrite.
-    apply f_eval_decl_complete in H2.
-    rewrite H2.
-    reflexivity.
-  - destruct IHeval_stmt as [k IH].
-    exists (S k).
-    simpl.
-    subst.
-    apply f_eval_decl_complete in H2.
-    repeat apply_rewrite.
-    rewrite H2.
-    apply_rewrite.
-  - destruct IHeval_stmt as [k IH].
-    exists (S k).
-    simpl.
-    subst.
-    repeat apply_rewrite.
-    apply f_eval_decl_complete in H2.
-    rewrite H2.
-    repeat apply_rewrite.
-    repeat setoid_rewrite app_length.
-    assert ((Datatypes.length slocal +
-             (Datatypes.length prefix' + Datatypes.length s') -
-             (Datatypes.length prefix + Datatypes.length s))
-            = (Datatypes.length slocal)).
-    {  omega. }
-    rewrite H1.
-    rewrite H6.
-    
-    rewrite (split2_complete _ _ _ (slocal ++ prefix' ++ s') slocal prefix' s').
-    + apply copy_out_correct.
-      assumption.
-    + reflexivity.
-    + reflexivity.
-    + reflexivity.
-Qed.
-
-(**********************************************************************)
-(**********************************************************************)
-
-(** * Subprogram Semantics *)
-
-(** In the current SPARK subset, there is no procedure call, 
-    so right now we only define the semantics for the main procedure.
-    And it can be used to test the tool chain from SPARK source code 
-    to Coq evaluation; Later, we will add the procedure call and 
-    modify the following procedure semantics;
-*)
-
-(** all declared variables in the same procedure should have unique 
-    names; 
-*)
-
-(** relational (eval_decl) and functional (f_eval_decl) semantics for 
-    variable declaration;
-*)
-
-(** for any initial state s, after executing the declaration d, 
-    it either returns a normal state s' or a run time error;
-    (for any variable declaration, if its initialization expression 
-     fails the run time checks, for example division by zero or overflow, 
-     then it returns an exception)
-*)
-
-Lemma eval_decl_state : forall s d s',
-        eval_decl s d s' -> (* s' is either a normal state or a run time error *)
-            (exists t, s' = S_Normal t) \/ s' = S_Run_Time_Error.
-Proof.
-    intros s d s' h.
-    induction h;
-    try match goal with
-    | [ |- (exists t, S_Normal ?t1 = S_Normal t) \/ _ ] => left; exists t1; reflexivity
-    | [ |- context [ _ \/ ?A = ?A ] ] => right; reflexivity
-    end; auto.
-Qed.
-
-
-(** f_eval_decl completeness and correctness proofs *)
-
-(** bisimulation proof between f_eval_decl and eval_decl: 
-    - f_eval_decl_correct
-    - f_eval_decl_complete
-*)
-
-Lemma f_eval_decl_correct_: forall d s s',
-    (f_eval_decl s d = (S_Normal s') -> eval_decl s d (S_Normal s')) /\
-    (f_eval_decl s d = S_Run_Time_Error -> eval_decl s d S_Run_Time_Error).
-Proof.
-    intros d s.
-    intros s'.
-    split;intro h.
-    - apply f_eval_decl_correct.
-      assumption.
-    - apply f_eval_decl_correct2.
-      assumption.
-Qed.
-
-
-(* = = = = = = Subprogram Body = = = = = =  *)
-(** relational and functional semantics for procedure body; *)
-(* Is this still needed for global procedures? probably not. *)
-Inductive eval_proc: store -> procedure_body -> state -> Prop :=
-    | eval_Proc_E: forall f s,
-        eval_decl s (procedure_declarative_part f) S_Run_Time_Error ->
-        eval_proc s f S_Run_Time_Error
-    | eval_Proc: forall f s1 s2 s3,
-        eval_decl s1 (procedure_declarative_part f) (S_Normal s2) ->
-        eval_stmt s2 (procedure_statements f) s3 ->
-        eval_proc s1 f s3.
-
-Function f_eval_proc k (s: store) (f: procedure_body): state :=
-    match (f_eval_decl s (procedure_declarative_part f)) with
-    | S_Normal s' => f_eval_stmt k s' (procedure_statements f)
-    | S_Run_Time_Error => S_Run_Time_Error
-    | _ => S_Abnormal
-    end.
-
-
-(** ** Main Procedure Evaluation Without Parameters *)
-
-(** relational and functional semantics for main procedure; *)
-
-Inductive eval_subprogram: store -> subprogram -> state -> Prop :=
-    | eval_Procedure: forall s s' ast_num f,
-        eval_proc s f s' ->
-        eval_subprogram s (Global_Procedure ast_num f) s'.
-
-Function f_eval_subprogram k (s: store) (f: subprogram): state := 
-    match f with 
-    | Global_Procedure ast_num f' => f_eval_proc k s f'
-    end.
-
-(** ** Bisimulation Between Relational And Functional Semantics For Main Procedure *)
-
-(** *** f_eval_subprogram_correct *)
-Theorem f_eval_subprogram_correct: forall k s f s',
-    (f_eval_subprogram k s f = S_Normal s' -> 
-        eval_subprogram s f (S_Normal s')) /\
-    (f_eval_subprogram k s f = S_Run_Time_Error -> 
-        eval_subprogram s f S_Run_Time_Error).
-Proof.
-    intros; 
-    split; intros;
-    destruct f;
-    simpl in H;
-    constructor;
-    unfold f_eval_proc in H;
-    remember (f_eval_decl s (procedure_declarative_part p)) as x;
-    symmetry in Heqx.
-  - (* normal state *)
-    destruct x; inversion H; subst.
-    econstructor.
-    + apply f_eval_decl_correct in Heqx.
-       apply Heqx.
-    + apply f_eval_stmt_correct in H.
-       rewrite H1; auto.
-  - (* run time error *)
-    destruct x; inversion H; subst.
-    + econstructor.
-       * apply f_eval_decl_correct in Heqx.
-         apply Heqx.
-       * rewrite H.
-         apply f_eval_stmt_correct in H; auto.
-    + econstructor.
-      apply f_eval_decl_correct2 in Heqx; auto.
-Qed.
-
-(** *** f_eval_subprogram_complete *)
-Theorem f_eval_subprogram_complete: forall s f s',
-    eval_subprogram s f s' ->
-    exists k, f_eval_subprogram k s f = s'.
-Proof.
-    intros s f s' h.
-    unfold f_eval_subprogram.
-    unfold f_eval_proc.
-    inversion h; subst.
-    inversion H; subst.
-  - apply f_eval_decl_complete in H0.
-    rewrite H0. 
-    exists 0; auto.
-  - apply f_eval_decl_complete in H0.
-    rewrite H0.
-    apply f_eval_stmt_complete in H1.
-    auto.
-Qed.
-
